Changes

Proofs/Spec.GC_part01.fsti
@@ -148,11 +148,23 @@ let max_tag = Usize.sub (Usize.shift_left 1UL 8ul) 1UL
 
 (*---------------------------------------------------------------------------------------------------------------------*)
 (*max_wosize, max_color, max_tag properties*)
-val max_wosize_lemma : unit -> Lemma (Usize.v max_wosize = pow2 54 - 1)
+let max_wosize_lemma () : Lemma (ensures (Usize.v max_wosize = pow2 54 - 1)) =
+  assert (Usize.v (Usize.shift_left 1UL 54ul) == pow2 54 % pow2 64);
+   Math.Lemmas.pow2_lt_compat 64 54;
+   Math.Lemmas.small_mod (pow2 54) (pow2 64)
 
-val max_color_size_lemma : unit -> Lemma (Usize.v max_color = pow2 2 - 1)
+let max_color_size_lemma () :Lemma (ensures (Usize.v max_color = pow2 2 - 1)) =
+   assert (Usize.v (Usize.shift_left 1UL 2ul) == pow2 2 % pow2 64);
+   Math.Lemmas.pow2_lt_compat 64 2;
+   Math.Lemmas.small_mod (pow2 2) (pow2 64)
 
-val max_tag_size_lemma : unit -> Lemma (Usize.v max_tag = pow2 8 - 1)
+
+
+let max_tag_size_lemma  () :Lemma (ensures (Usize.v max_tag = pow2 8 - 1)) =
+   assert (Usize.v (Usize.shift_left 1UL 8ul) == pow2 8 % pow2 64);
+   Math.Lemmas.pow2_lt_compat 64 8;
+   Math.Lemmas.small_mod (pow2 8) (pow2 64)
+
 (*---------------------------------------------------------------------------------------------------------------------*)
 
 (*Definitions*)
@@ -164,9 +176,10 @@ type color = cl:Usize.t{0 <= Usize.v cl /\ Usize.v cl <= Usize.v max_color}
 
 type tag = tg:Usize.t{0 <= Usize.v tg /\ Usize.v tg <= Usize.v max_tag}
 
-val is_size_fits_after_subtraction :(x:Usize.t) ->
-                                    (y:Usize.t) ->
-                       Tot (b:bool{b == true <==> UInt.fits (Usize.v x - Usize.v y) Usize.n})
+let is_size_fits_after_subtraction (x:Usize.t)
+                                   (y:Usize.t)
+                       : Tot (b:bool{b == true <==> UInt.fits (Usize.v x - Usize.v y) Usize.n}) =
+  UInt.fits (Usize.v x - Usize.v y) Usize.n
 
 type hp_addr = h:Usize.t {Usize.v h >= 0 /\ Usize.v h < heap_size /\ (Usize.v h % 8 == 0)}
 
@@ -381,53 +394,225 @@ write_word_after_start_end_lemma byte_array byte_index value;
 
 
 /// Extract wosize from header value
-val getWosize : (h:Usize.t) ->
-          Tot (wz:wosize{wz == Usize.shift_right h 10ul})
+let getWosize (h:Usize.t)
+          :Tot (wz:wosize{wz == Usize.shift_right h 10ul}) =
+ let _ = max_wosize_lemma () in
+ let _ = assert (Usize.v max_wosize = pow2 54 - 1) in
+ let wz = Usize.shift_right h 10ul in
+ assert (Usize.v wz == Usize.v h/ pow2 10);
+ assert (Usize.v wz <= Usize.v max_wosize);
+ assert (Usize.v wz >= 0);
+ wz
+
 
 /// Extract color from header value
-val getColor : (h:Usize.t) ->
-          Tot (c:color{c = Usize.logand (Usize.shift_right h 8ul) 3UL})
+let getColor  (h:Usize.t)
+          : Tot (c:color{c = Usize.logand (Usize.shift_right h 8ul) 3UL}) =
+ let _ = max_color_size_lemma () in
+ let _ = assert (Usize.v max_color = pow2 2 - 1) in
+ let c' = Usize.shift_right h 8ul in
+ let c = Usize.logand c' 3UL in
+ assert (Usize.v c' == Usize.v h/ pow2 8);
+ assert (Usize.v c' <= pow2 64/pow2 8);
+ Math.Lemmas.pow2_minus 64 8;
+ assert (Usize.v c' <= pow2 56);
+ UInt.logand_le #64 (Usize.v c') 3;
+ assert (Usize.v c <= Usize.v c');
+
+ assert (Usize.v c <= Usize.v max_color);
+ assert (Usize.v  h <= UInt.max_int 64);
+ assert (Usize.v h <= pow2 64 - 1);
+ assert (Usize.v c <=  pow2 64 - 1);
+ assert (Usize.v max_color <= pow2 64 - 1);
+ c
+
 
 /// Extract tag from header value
-val getTag : (h:Usize.t) ->
-          Tot (tg:tag{tg == Usize.logand h 255UL})
-
-val color_of_object1 : (v_id: hp_addr) ->
-                       (g:heap)->
-             Tot (c:color{c == getColor(read_word g v_id)}) 
-
-val wosize_of_object1 : (v_id: hp_addr) ->
-                        (g:heap)->
-             Tot (w:wosize{w == getWosize(read_word g v_id)}) 
-
-
-val tag_of_object1 : (v_id: hp_addr) ->
-                     (g:heap)->
-             Tot (t:tag{t == getTag(read_word g v_id)}) 
+let getTag  (h:Usize.t) 
+          : Tot (tg:tag{tg == Usize.logand h 255UL}) =
+ let _ = max_tag_size_lemma () in
+ assert (Usize.v max_tag = pow2 8 - 1);
+ let t = Usize.logand h 255UL in
+ UInt.logand_le #64 (Usize.v h) 255;
+ assert (Usize.v max_tag <= pow2 8 - 1);
+ assert (Usize.v t <= 255);
+ assert (Usize.v t <= Usize.v max_tag);
+ t
 
 
-val isBlueObject1 :(v_id: hp_addr)->
-                   (g:heap) ->
-         Tot (b: bool {b == true <==> (color_of_object1 v_id g) == blue}) 
+let color_of_object1   (v_id: hp_addr)
+                       (g:heap)
+             : Tot (c:color{c == getColor(read_word g v_id)})  =
+  let hd_val = read_word g v_id in
+  let c = getColor (hd_val) in
+  c
 
-val isWhiteObject1 : (v_id: hp_addr)->
-                     (g:heap) ->
-         Tot (b: bool {b == true <==> (color_of_object1 v_id g) == white}) 
 
-val isGrayObject1 : (v_id: hp_addr)->
-                    (g:heap) ->
-         Tot (b: bool {b == true <==> (color_of_object1 v_id g) == gray}) 
+let wosize_of_object1 (v_id: hp_addr) 
+                        (g:heap)
+             :Tot (w:wosize{w == getWosize(read_word g v_id)}) =
+  let hd_val = read_word g v_id in
+  let w = getWosize (hd_val) in
+  w
 
-val isBlackObject1 : (v_id: hp_addr)->
-                     (g:heap) ->
-         Tot (b: bool {b == true <==> (color_of_object1 v_id g) == black}) 
 
-val makeHeader : (wz:wosize) ->
-                 (c:color) ->
-                 (tg:tag) ->
-             Tot (h:Usize.t{wz == getWosize h /\
+let tag_of_object1   (v_id: hp_addr)
+                     (g:heap)
+             :Tot (t:tag{t == getTag(read_word g v_id)}) =
+  let hd_val = read_word g v_id in
+  let t = getTag (hd_val) in
+  t
+
+let isBlueObject1  (v_id: hp_addr)
+                   (g:heap) 
+        :Tot (b: bool {b == true <==> (color_of_object1 v_id g) == blue}) =
+ if color_of_object1 v_id g = blue then true
+ else
+  false
+
+let isWhiteObject1  (v_id: hp_addr)
+                     (g:heap) 
+        : Tot (b: bool {b == true <==> (color_of_object1 v_id g) == white}) =
+  if color_of_object1 v_id g = white then true
+ else
+  false
+
+let isGrayObject1   (v_id: hp_addr)
+                    (g:heap)
+        : Tot (b: bool {b == true <==> (color_of_object1 v_id g) == gray}) =
+  if color_of_object1 v_id g = gray then true
+ else
+  false
+
+let isBlackObject1   (v_id: hp_addr)
+                     (g:heap) 
+        : Tot (b: bool {b == true <==> (color_of_object1 v_id g) == black}) =
+ if color_of_object1 v_id g = black then true
+ else
+  false
+
+open FStar.FunctionalExtensionality
+open FStar.UInt
+
+#push-options "--z3rlimit 500 --fuel 0 --ifuel 1" (*Be careful to use this. Always set fuel limits to default or higher if
+                                                 recursive calls dont work as expected*)
+
+#push-options "--split_queries always"
+
+#restart-solver
+
+let makeHeader   (wz:wosize)
+                 (c:color)
+                 (tg:tag) 
+             :Tot (h:Usize.t{wz == getWosize h /\
                             c == getColor h /\
-                            tg == getTag h})
+                            tg == getTag h}) =
+ let l1 = Usize.shift_left wz 10ul in
+ let l2 = Usize.shift_left c 8ul in
+ let l3 = Usize.shift_left tg 0ul in
+ assert (Usize.v l1 == Usize.v wz * pow2 10 % pow2 64);
+
+ //First prove wz, c and tag are less than the power of maximum shift needed to create max_wosize, max_color and max_tag
+ max_wosize_lemma();
+ max_color_size_lemma();
+ max_tag_size_lemma ();
+ assert (Usize.v wz < pow2 54);
+ assert (Usize.v c < pow2 2);
+ assert (Usize.v tg < pow2 8);
+
+ //Prove that wz shifted to left 10 positions is less than pow2 32. So when we take mod of pow2 32, the shift will not overflow
+// Math.Lemmas.lemma_mult_lt_right (pow2 10) (Usize.v wz) (pow2 22);
+ assert (pow2 10 > 0);
+ assert ((Usize.v wz) <  (pow2 54));
+ assert ((Usize.v wz) * pow2 10 < pow2 54 * pow2 10);
+ Math.Lemmas.pow2_plus 54 10;
+ assert (Usize.v wz * pow2 10 < pow2 64);
+// Math.Lemmas.small_mod (Usize.v wz * pow2 10) (pow2 32);
+ assert (Usize.v l1 == Usize.v wz * pow2 10);
+
+
+ assert (Usize.v l2 == Usize.v c * pow2 8);
+ assert (Usize.v l3 == Usize.v tg * pow2 0);
+
+ let s = Usize.add (Usize.add l1 l2) l3 in
+ assert (Usize.v s < pow2 64);
+ assert (Usize.v l1 < pow2 64);
+ assert (Usize.v l2 < pow2 64);
+ assert (Usize.v l3 < pow2 64);
+
+ let l1' = Usize.shift_right l1 10ul in
+ let l2' = Usize.shift_right l2 10ul in
+ let l3' = Usize.shift_right l3 10ul in
+ assert (Usize.v l1' == Usize.v l1 /pow2 10);
+ assert (Usize.v l2' == Usize.v l2 /pow2 10);
+ assert (Usize.v l3' == Usize.v l3 /pow2 10);
+
+ assert (Usize.v l1' == (Usize.v wz * pow2 10)/pow2 10);
+ Math.Lemmas.cancel_mul_div (Usize.v wz) (pow2 10);
+ assert (Usize.v l1' == Usize.v wz);
+
+ assert (Usize.v l2' == Usize.v c * (pow2 8/pow2 10));
+
+ assert (pow2 8 < pow2 10);
+ assert (Usize.v l3' == Usize.v tg * (pow2 0/pow2 10));
+ let s1' =  Usize.shift_right s 10ul in
+ assert (s1' == getWosize s);
+ assert (Usize.v s1' == Usize.v l1' + Usize.v l2' + Usize.v l3');
+ assert (Usize.v s1' == Usize.v wz);
+ assert (getWosize s == wz);
+
+ let s2 = Usize.shift_right s 8ul in
+
+ let l1'' = Usize.shift_right l1 8ul in
+ let l2'' = Usize.shift_right l2 8ul in
+ let l3'' = Usize.shift_right l3 8ul in
+ assert (Usize.v l1'' == Usize.v l1 /pow2 8);
+ assert (Usize.v l2'' == Usize.v l2 /pow2 8);
+ assert (Usize.v l3'' == Usize.v l3 /pow2 8);
+
+ assert (Usize.v l1'' == (Usize.v wz * pow2 10)/pow2 8);
+ Math.Lemmas.pow2_minus 10 8;
+ assert (Usize.v l1'' == Usize.v wz * pow2 2);
+
+ assert (Usize.v l2'' == (Usize.v c * pow2 8 )/pow2 8);
+ Math.Lemmas.cancel_mul_div (Usize.v c) (pow2 8);
+ assert (Usize.v l2'' == Usize.v c);
+
+ assert (Usize.v l3'' == (Usize.v tg * pow2 0)/pow2 8);
+ assert (Usize.v l3'' == 0);
+
+ assert (Usize.v s == Usize.v l1 + Usize.v l2 + Usize.v l3);
+ assert (s2 == Usize.shift_right s 8ul);
+ assert (Usize.v s2 == (Usize.v l1 + Usize.v l2 + Usize.v l3)/pow2 8);
+ assert (Usize.v s2 == (Usize.v wz * pow2 10 + Usize.v c * pow2 8 + Usize.v tg * pow2 0)/pow2 8);
+ assert (Usize.v s2 == ((Usize.v wz * pow2 10)/pow2 8) + ((Usize.v c * pow2 8)/pow2 8) + ((Usize.v tg * pow2 0)/pow2 8));
+ assert (Usize.v s2 == ((Usize.v wz * pow2 10)/pow2 8) + ((Usize.v c * pow2 8)/pow2 8));
+ assert (Usize.v s2 == ((Usize.v wz * pow2 10)/pow2 8) + Usize.v c);
+ assert (Usize.v s2 == (Usize.v wz * pow2 2) + Usize.v c);
+
+ //assert (Usize.v s2 == Usize.v l1'' + Usize.v l2'' + Usize.v l3'');
+
+ let s2' = Usize.logand s2 3UL in
+
+ assert (pow2 2 - 1 == 3);
+ logand_mask #64 (Usize.v s2) 2;
+ assert (Usize.v s2' == Usize.v s2 % pow2 2);
+ assert (Usize.v c < pow2 2);
+ assert ((Usize.v wz * pow2 2) % pow2 2 == 0);
+ assert (Usize.v s2' == Usize.v c);
+
+ let s3' = Usize.logand s 255UL in
+ logand_mask #64 (Usize.v s) 8;
+
+ assert (s2' == c);
+ assert (s3' == tg);
+ assert (getColor s == s2');
+ assert (getTag s == s3');
+ assert (getColor s == c);
+ assert (getTag s == tg);
+
+ s
+
 /// -----------------------------------------------------------------------------------------------------------------------------------------------------------------
 /// h_index = start byte address of the object
 /// wz = wosize type
@@ -443,10 +628,18 @@ val makeHeader : (wz:wosize) ->
 ///      header                    field 1        heap_size
 /// -----------------------------------------------------------------------------------------------------------------------------------------------------------------
 
+#pop-options
 
-val isPointer : (v_id: hp_addr) ->
-                (g:heap) ->
-            Tot (b:bool{b == true <==> Usize.logand (read_word g v_id) 1UL == 0UL})
+#pop-options
+
+#push-options "--z3rlimit 100 --fuel 2 --ifuel 1"
+
+
+let isPointer   (v_id: hp_addr) 
+                (g:heap) 
+           : Tot (b:bool{b == true <==> Usize.logand (read_word g v_id) 1UL == 0UL}) =
+ if Usize.logand (read_word g v_id) 1UL = 0UL then true else false
+
 
 (*No object size exceeds the heap limit*)
 (*h_index + (wz + 1) * mword takes to the next header. Therefore, (Usize.v h_index + (((Usize.v wz + 1) * Usize.v mword) - 1) will take us to the last index of the
@@ -470,22 +663,53 @@ let closinfo_val  (g:heap)
 (*The sum of an address and its ((wosize value + 1) * mword - 1) should be less than the heap_size*)
 (*(wosize value + 1) * mword ---> Takes to the heap address next of wosize value in the byte array.*)
 
-val is_fields_within_limit1  : (h_index: hp_addr) ->
-                               (wz: wosize)->
-              Tot (b:bool{b == true <==> (Usize.v h_index + (((Usize.v wz + 1) * Usize.v mword) - 1) < heap_size)})
+let is_fields_within_limit1   (h_index: hp_addr) 
+                               (wz: wosize)
+              :Tot (b:bool{b == true <==> (Usize.v h_index + (((Usize.v wz + 1) * Usize.v mword) - 1) < heap_size)}) =
+//let s = Usize.add h_index (Usize.mul wz mword) in
+ let s1 = Usize.add wz 1UL in // s1 = (wz + 1)
+ let s2 = Usize.mul s1 mword in //s2 = (s1 * mword)
+ let s3 = Usize.sub s2 1UL in // s3 = s2 - 1 = (s1 * mword) - 1 = ((wz + 1) * mword) - 1
+ let s =  Usize.add h_index s3 in // s = h_index + s3 = h_index + ((wz + 1) * mword) - 1
+ if (Usize.v s < heap_size) then
+    true
+  else
+    false
+
 
 #push-options "--split_queries always"
 
 
-val is_fields_contents_within_limit2 : (h_index: hp_addr) ->
-                                       (wz: wosize{is_fields_within_limit1 h_index wz}) ->
-                                       (g:heap(*{Usize.v (tag_of_object1 h_index g) < no_scan_tag /\
-                                               Usize.v (tag_of_object1 h_index g) <> closure_tag}*)) ->
-                            Tot (b:bool{b == true <==>  (forall (i:Usize.t {Usize.v i > 0 /\ Usize.v i <= Usize.v wz}).isPointer (Usize.add h_index (Usize.mul i mword)) g ==>
+let rec is_fields_contents_within_limit2 (h_index: hp_addr) 
+                                         (wz: wosize{is_fields_within_limit1 h_index wz}) 
+                                         (g:heap(*{Usize.v (tag_of_object1 h_index g) < no_scan_tag /\
+                                               Usize.v (tag_of_object1 h_index g) <> closure_tag}*)) 
+                           :Tot (b:bool{b == true <==>  (forall (i:Usize.t {Usize.v i > 0 /\ Usize.v i <= Usize.v wz}).isPointer (Usize.add h_index (Usize.mul i mword)) g ==>
                                                           (Usize.v (read_word g (Usize.add h_index (Usize.mul i mword))) >= Usize.v mword /\
                                                           Usize.v (read_word g (Usize.add h_index (Usize.mul i mword))) < heap_size) /\
                                                           is_hp_addr (read_word g (Usize.add h_index (Usize.mul i mword))))})
-                            (decreases (Usize.v wz))
+                            (decreases (Usize.v wz)) =
+  if (Usize.v wz = 0) then true
+    else
+      (
+        assert (Usize.v wz > 0);
+        let s = Usize.add h_index (Usize.mul wz mword) in
+        let wz' = Usize.sub wz 1UL in
+        if (isPointer s g) then
+        (
+          let succ = read_word g s in
+          if Usize.v succ >= Usize.v mword && Usize.v succ < heap_size && is_hp_addr succ then
+           is_fields_contents_within_limit2 h_index wz' g
+          else
+           false
+        )
+        else
+        (
+          is_fields_contents_within_limit2 h_index wz' g
+        )
+       )
+
+
 
 let wosize_times_mword_multiple_of_mword (wz:wosize)
                      :Lemma 
@@ -497,9 +721,24 @@ let sum_of_multiple_of_mword_is_multiple_of_mword (x:Usize.t{Usize.v x % Usize.v
                                 :Lemma 
                                  (ensures ((Usize.v x + Usize.v y) % Usize.v mword == 0)) = ()
 
-val objects2 : (h_index: hp_addr)->
-               (g:heap) ->
-        Tot (s:seq Usize.t {Seq.length s > 0 ==> (forall x. Seq.mem x s ==> Usize.v x >= 0 /\ Usize.v x < heap_size) /\
+let color_lemma (h_index)
+                (g:heap)
+          : Lemma
+            (ensures ((color_of_object1 h_index g == white) \/
+                      (color_of_object1 h_index g == black) \/
+                      (color_of_object1 h_index g == gray) \/
+                      (color_of_object1 h_index g == blue))) = ()
+
+#push-options "--split_queries always "
+
+#restart-solver
+
+#restart-solver
+
+
+let rec objects2   (h_index: hp_addr)
+               (g:heap) 
+       : Tot (s:seq Usize.t {Seq.length s > 0 ==> (forall x. Seq.mem x s ==> Usize.v x >= 0 /\ Usize.v x < heap_size) /\
                                                  (forall x. Seq.mem x s ==> Usize.v x % Usize.v mword == 0) /\
                                                  (Seq.mem h_index s) (*/\
                                                  (let h_index_new =  
@@ -517,7 +756,67 @@ val objects2 : (h_index: hp_addr)->
                                                    (Usize.v y <= Usize.v x + (((Usize.v (getWosize (read_word g x)) + 1) * Usize.v mword) - 1)) ==>
                                                    ~(Seq.mem y s)))})
                                                                      
-                       (decreases (heap_size - Usize.v h_index))
+                       (decreases (heap_size - Usize.v h_index)) =
+  let wz =  getWosize (read_word g h_index) in
+let h_index_new =  Usize.add h_index (Usize.mul (Usize.add wz 1UL) mword) in
+if Usize.v wz = 0 then
+(
+  let f' = Seq.empty  in// There are no zero length objects.
+  assert (Seq.length f' > 0 /\ (Usize.v h_index_new < heap_size) ==> Seq.mem h_index_new f');
+  assert (forall x. Seq.mem x f' ==> is_hp_addr x);
+  f'
+)
+else
+(
+  let h_index_new =  Usize.add h_index (Usize.mul (Usize.add wz 1UL) mword) in // possible next header = h_index + (wz + 1) * mword. Eg. h_index = 0; wz = 1; mword = 8;
+                                                                               // h_index_new = 0 + (1 + 1) * 8 = 0 + 16 = 16. h_index range in g = 0......7
+                                                                               // first field range in g = 8......15. Only one field. So next header starts at 16
+  if Usize.v h_index_new <= heap_size then //valid heap condition
+  (
+    if Usize.v h_index_new = heap_size then // h_index_new == heap_size --> The last block is h_index, So just create a singleton with h_index and return.
+    (
+       assert (Usize.v h_index_new == heap_size);
+       let f = Seq.create 1 h_index in
+
+       G.is_vertex_set_lemma2 f;
+       assert (Seq.length f > 0 /\ (Usize.v h_index_new < heap_size) ==> Seq.mem h_index_new f);
+       assert (forall x. Seq.mem x f ==> is_hp_addr x);
+       f
+    )
+    else
+    (
+      assert (Usize.v h_index_new < heap_size);
+      let f_index_new =  Usize.add h_index_new mword in
+      let f' =  objects2 h_index_new g in
+      if length f' = 0 ||  (Usize.v f_index_new = heap_size) then
+      (
+        assert (Seq.length f' > 0 /\ (Usize.v h_index_new < heap_size) ==> Seq.mem h_index_new f');
+        assert (forall x. Seq.mem x f' ==> is_hp_addr x);
+        f'
+      )
+       else
+       (
+         assert (Usize.v h_index_new < heap_size);
+         lemma_tl h_index f';
+         let f'' = cons h_index f' in
+         assert (Seq.length f'' > 0 /\ (Usize.v h_index_new < heap_size) ==> Seq.mem h_index_new f'');
+         G.is_vertex_set_cons h_index f';
+         assert (G.is_vertex_set f'');
+         assert (forall x. Seq.mem x f'' ==> is_hp_addr x);
+         f''
+       )
+    )
+  )
+  else
+  (
+    assert (Usize.v h_index_new > heap_size); //h_index_new is greater than heap_size means the last object size exceeds the heap.
+    let f' = Seq.empty in
+    assert (Seq.length f' > 0 /\ (Usize.v h_index_new < heap_size) ==> Seq.mem h_index_new f');
+    assert (forall x. Seq.mem x f' ==> is_hp_addr x);
+    f'
+  )
+)
+
 
 /// Given the start address of an object, which is the address of the first field of the object, hd_address gets the header address of that object
 let hd_address (st_index: hp_addr{UInt.fits (Usize.v st_index - Usize.v mword) Usize.n})
@@ -530,15 +829,18 @@ let hd_address (st_index: hp_addr{UInt.fits (Usize.v st_index - Usize.v mword) U
 
 #restart-solver 
 
-val objects2_wosize_lemma : (h_index: hp_addr)->
-                           (g:heap) ->
-                 Lemma
-                  (ensures (Seq.length (objects2 h_index g) > 0) ==> Usize.v (getWosize (read_word g h_index)) > 0)
+let objects2_wosize_lemma  (h_index: hp_addr)
+                           (g:heap)
+                : Lemma
+                  (ensures (Seq.length (objects2 h_index g) > 0) ==> Usize.v (getWosize (read_word g h_index)) > 0) =
+  ()
 
 
-val objects2_empty_lemma : (h_index: hp_addr)->
-                           (g:heap) ->
-                Lemma
+
+
+let objects2_empty_lemma   (h_index: hp_addr)
+                           (g:heap)
+              :Lemma
                 (requires (let wz = getWosize (read_word g h_index) in
                            let h_index_new = Usize.add h_index (Usize.mul (Usize.add wz 1UL) mword) in
                            ( Usize.v wz > 0 /\
@@ -549,11 +851,12 @@ val objects2_empty_lemma : (h_index: hp_addr)->
                           (Seq.length (objects2 h_index_new g) == 0 ==>
                           (objects2 h_index g) == (objects2 h_index_new g))
                          )
-                )
+                ) =
+ ()
 
-val objects2_non_empty_lemma : (h_index: hp_addr)->
-                           (g:heap) ->
-                Lemma
+let objects2_non_empty_lemma  (h_index: hp_addr)
+                              (g:heap)
+                :Lemma
                 (requires (let wz = getWosize (read_word g h_index) in
                            let h_index_new = Usize.add h_index (Usize.mul (Usize.add wz 1UL) mword) in
                            (Usize.v wz > 0 /\
@@ -564,16 +867,18 @@ val objects2_non_empty_lemma : (h_index: hp_addr)->
                           (Seq.length (objects2 h_index_new g) > 0 ==>
                           (objects2 h_index g) == Seq.cons h_index (objects2 h_index_new g))
                          )
-                )
+                ) = ()
 
-val objects2_singleton_lemma : (h_index: hp_addr)->
-                           (g:heap) ->
-                Lemma
+
+
+let objects2_singleton_lemma  (h_index: hp_addr)
+                              (g:heap)
+               : Lemma
                 (requires (let wz = getWosize (read_word g h_index) in
                            let h_index_new = Usize.add h_index (Usize.mul (Usize.add wz 1UL) mword) in
                            (Usize.v wz > 0 /\
                             Usize.v h_index_new == heap_size)))
-                (ensures ((objects2 h_index g) == Seq.create 1 h_index))
+                (ensures ((objects2 h_index g) == Seq.create 1 h_index)) = ()
 
 
 
@@ -626,53 +931,547 @@ let extract_start_env_bits (clos_info:Usize.t)
  r1
 
 #restart-solver 
+let wosize_plus_times_mword_multiple_of_mword (wz:wosize)
+                     :Lemma
+                      (ensures (Usize.v (Usize.mul (Usize.add wz 1UL) mword) % Usize.v mword == 0)) = ()
 
-val objects2_mem_lemma1 :   (h_index: hp_addr) ->
-                            (g:heap) ->
+let objects2_mem_lemma (h_index: hp_addr)
+                           (g:heap)
+
+
+          : Lemma
+            (ensures (let wz =  getWosize (read_word g h_index) in
+                      let h_index_new =  Usize.add h_index (Usize.mul (Usize.add wz 1UL) mword) in
+                      (Seq.length (objects2 h_index g) > 0 /\ (Usize.v h_index_new < heap_size) ==> Seq.mem h_index_new (objects2 h_index g))))
+            (decreases (heap_size - Usize.v h_index)) =
+let wz =  getWosize (read_word g h_index) in
+let h_index_new =  Usize.add h_index (Usize.mul (Usize.add wz 1UL) mword) in
+if Usize.v wz = 0 then
+(
+  let f' = Seq.empty  in// There are no zero length objects.
+  assert (Seq.length f' > 0 /\ (Usize.v h_index_new < heap_size) ==> Seq.mem h_index_new f');
+  ()
+)
+else
+(
+  let h_index_new =  Usize.add h_index (Usize.mul (Usize.add wz 1UL) mword) in // possible next header = h_index + (wz + 1) * mword. Eg. h_index = 0; wz = 1; mword = 8;
+                                                                               // h_index_new = 0 + (1 + 1) * 8 = 0 + 16 = 16. h_index range in g = 0......7
+                                                                               // first field range in g = 8......15. Only one field. So next header starts at 16
+  if Usize.v h_index_new <= heap_size then //valid heap condition
+  (
+    if Usize.v h_index_new = heap_size then // h_index_new == heap_size --> The last block is h_index, So just create a singleton with h_index and return.
+    (
+       assert (Usize.v h_index_new == heap_size);
+       let f = Seq.create 1 h_index in
+
+       G.is_vertex_set_lemma2 f;
+       assert (Seq.length f > 0 /\ (Usize.v h_index_new < heap_size) ==> Seq.mem h_index_new f);
+       ()
+    )
+    else
+    (
+      assert (Usize.v h_index_new < heap_size); // h_index_new < heap_size, still more blocks to explore, hence recurse.
+      wosize_plus_times_mword_multiple_of_mword wz;
+      sum_of_multiple_of_mword_is_multiple_of_mword h_index (Usize.mul (Usize.add wz 1UL) mword);
+      assert (Usize.v h_index_new % Usize.v mword == 0);
+      assert (is_hp_addr h_index_new);
+      let f' =  objects2 h_index_new g in
+      if length f' = 0 then
+      (
+        assert (Seq.length f' > 0 /\ (Usize.v h_index_new < heap_size) ==> Seq.mem h_index_new f');
+        ()
+      )
+       else
+       (
+
+         lemma_tl h_index f';
+         let f'' = cons h_index f' in
+
+         G.is_vertex_set_cons h_index f';
+         assert (Seq.length f'' > 0 /\ (Usize.v h_index_new < heap_size) ==> Seq.mem h_index_new f'');
+         ()
+       )
+    )
+  )
+  else
+  (
+    assert (Usize.v h_index_new > heap_size); //h_index_new is greater than heap_size means the last object size exceeds the heap.
+    let f' = Seq.empty in
+    assert (Seq.length f' > 0 /\ (Usize.v h_index_new < heap_size) ==> Seq.mem h_index_new f');
+    ()
+  )
+)
+
+#restart-solver
+
+#restart-solver
+
+let rec objects2_mem_lemma1     (h_index: hp_addr) 
+                            (g:heap)
                            
                       
-            Lemma 
+           : Lemma 
             (ensures ((Seq.length (objects2 h_index g) > 0  ==> (forall x. Seq.mem x (objects2 h_index g) /\ 
                                                                   Usize.v (Usize.add x (Usize.mul (Usize.add (getWosize (read_word g x)) 1UL) mword)) < heap_size ==> 
                                                                        Seq.mem (Usize.add x (Usize.mul (Usize.add (getWosize (read_word g x)) 1UL) mword)) 
                                                                            (objects2 h_index g)))))
-            (decreases (heap_size - Usize.v h_index))
+            (decreases (heap_size - Usize.v h_index)) =
+let wz =  getWosize (read_word g h_index) in
+let h_index_new =  Usize.add h_index (Usize.mul (Usize.add wz 1UL) mword) in
+if Usize.v wz = 0 then
+(
+  let f' = Seq.empty  in// There are no zero length objects.
+  assert (Seq.length f' > 0 /\ (Usize.v h_index_new < heap_size) ==> Seq.mem h_index_new f');
+  assert (Seq.length (objects2 h_index g) > 0  ==> (forall x. Seq.mem x (objects2 h_index g) /\
+                                                                  Usize.v (Usize.add x (Usize.mul (Usize.add (getWosize (read_word g x)) 1UL) mword)) < heap_size ==>
+                                                                       Seq.mem (Usize.add x (Usize.mul (Usize.add (getWosize (read_word g x)) 1UL) mword))
+                                                                           (objects2 h_index g)));
+  ()
+)
+else
+(
+  let h_index_new =  Usize.add h_index (Usize.mul (Usize.add wz 1UL) mword) in // possible next header = h_index + (wz + 1) * mword. Eg. h_index = 0; wz = 1; mword = 8;
+                                                                               // h_index_new = 0 + (1 + 1) * 8 = 0 + 16 = 16. h_index range in g = 0......7
+                                                                               // first field range in g = 8......15. Only one field. So next header starts at 16
+  if Usize.v h_index_new <= heap_size then //valid heap condition
+  (
+    if Usize.v h_index_new = heap_size then // h_index_new == heap_size --> The last block is h_index, So just create a singleton with h_index and return.
+    (
+       assert (Usize.v h_index_new == heap_size);
+       let f = Seq.create 1 h_index in
 
-val objects2_equal_lemma :(h_index:hp_addr) ->
-                          (g:heap) ->
-                          (g':heap) ->
-                     Lemma
+       G.is_vertex_set_lemma2 f;
+       assert (Seq.length f > 0 /\ (Usize.v h_index_new < heap_size) ==> Seq.mem h_index_new f);
+       assert (Seq.length (objects2 h_index g) > 0  ==> (forall x. Seq.mem x (objects2 h_index g) /\
+                                                                  Usize.v (Usize.add x (Usize.mul (Usize.add (getWosize (read_word g x)) 1UL) mword)) < heap_size ==>
+                                                                       Seq.mem (Usize.add x (Usize.mul (Usize.add (getWosize (read_word g x)) 1UL) mword))
+                                                                           (objects2 h_index g)));
+       ()
+    )
+    else
+    (
+      assert (Usize.v h_index_new < heap_size); // h_index_new < heap_size, still more blocks to explore, hence recurse.
+      wosize_plus_times_mword_multiple_of_mword wz;
+      sum_of_multiple_of_mword_is_multiple_of_mword h_index (Usize.mul (Usize.add wz 1UL) mword);
+      assert (Usize.v h_index_new % Usize.v mword == 0);
+      assert (is_hp_addr h_index_new);
+      let f' =  objects2 h_index_new g in
+      objects2_mem_lemma1 h_index_new g;
+      if length f' = 0 then
+      (
+        assert (Seq.length f' > 0 /\ (Usize.v h_index_new < heap_size) ==> Seq.mem h_index_new f');
+        assert (Seq.length (objects2 h_index g) > 0  ==> (forall x. Seq.mem x (objects2 h_index g) /\
+                                                                  Usize.v (Usize.add x (Usize.mul (Usize.add (getWosize (read_word g x)) 1UL) mword)) < heap_size ==>
+                                                                       Seq.mem (Usize.add x (Usize.mul (Usize.add (getWosize (read_word g x)) 1UL) mword))
+                                                                           (objects2 h_index g)));
+        ()
+      )
+       else
+       (
+         lemma_tl h_index f';
+         let f'' = cons h_index f' in
+         assert (Seq.length f'' > 0 /\ (Usize.v h_index_new < heap_size) ==> Seq.mem h_index_new f'');
+         G.is_vertex_set_cons h_index f';
+         assert (Seq.length f'' > 0 /\ (Usize.v h_index_new < heap_size) ==> Seq.mem h_index_new f'');
+         assert (Seq.length (objects2 h_index g) > 0  ==> (forall x. Seq.mem x (objects2 h_index g) /\
+                                                                  Usize.v (Usize.add x (Usize.mul (Usize.add (getWosize (read_word g x)) 1UL) mword)) < heap_size ==>
+                                                                       Seq.mem (Usize.add x (Usize.mul (Usize.add (getWosize (read_word g x)) 1UL) mword))
+                                                                           (objects2 h_index g)));
+         ()
+       )
+    )
+  )
+  else
+  (
+    assert (Usize.v h_index_new > heap_size); //h_index_new is greater than heap_size means the last object size exceeds the heap.
+    let f' = Seq.empty in
+    assert (Seq.length f' > 0 /\ (Usize.v h_index_new < heap_size) ==> Seq.mem h_index_new f');
+    assert (Seq.length (objects2 h_index g) > 0  ==> (forall x. Seq.mem x (objects2 h_index g) /\
+                                                                  Usize.v (Usize.add x (Usize.mul (Usize.add (getWosize (read_word g x)) 1UL) mword)) < heap_size ==>
+                                                                       Seq.mem (Usize.add x (Usize.mul (Usize.add (getWosize (read_word g x)) 1UL) mword))
+                                                                           (objects2 h_index g)));
+    ()
+  )
+)
+
+
+
+let rec objects2_equal_lemma  (h_index:hp_addr) 
+                          (g:heap) 
+                          (g':heap) 
+                    : Lemma
                        (requires (forall (x:Usize.t{Usize.v x < heap_size /\ Usize.v x % 8 == 0}). getWosize (read_word g x) == getWosize (read_word g' x)))
                        (ensures objects2 h_index g == objects2 h_index g')
-                       (decreases (heap_size - Usize.v h_index))
+                       (decreases (heap_size - Usize.v h_index)) =
+ let wz =  getWosize (read_word g h_index) in
+
+if Usize.v wz = 0 then () // There are no zero length objects.
+else
+(
+  let h_index_new =  Usize.add h_index (Usize.mul (Usize.add wz 1UL) mword) in // possible next header = h_index + (wz + 1) * mword. Eg. h_index = 0; wz = 1; mword = 8;
+                                                                               // h_index_new = 0 + (1 + 1) * 8 = 0 + 16 = 16. h_index range in g = 0......7
+                                                                               // first field range in g = 8......15. Only one field. So next header starts at 16
+  if Usize.v h_index_new <= heap_size then //valid heap condition
+  (
+    if Usize.v h_index_new = heap_size then // h_index_new == heap_size --> The last block is h_index, So just create a singleton with h_index and return.
+    (
+       assert (Usize.v h_index_new == heap_size);
+       let f = Seq.create 1 h_index in
+
+       G.is_vertex_set_lemma2 f;
+       ()
+    )
+    else
+    (
+      assert (Usize.v h_index_new < heap_size); // h_index_new < heap_size, still more blocks to explore, hence recurse.
+      let f' =  objects2 h_index_new g in
+      objects2_equal_lemma h_index_new g g';
+      if length f' = 0 then ()
+       else
+       (
+         (*lemma_tail_snoc f' h_index;
+         lemma_mem_snoc f' h_index;
+         let f'' = snoc f' h_index in
+
+         G.snoc_unique_lemma h_index f';*)
+         lemma_tl h_index f';
+         let f'' = cons h_index f' in
+         assert (Seq.length f'' > 0 /\ (Usize.v h_index_new < heap_size) ==> Seq.mem h_index_new f'');
+         G.is_vertex_set_cons h_index f';
+
+         ()
+       )
+    )
+  )
+  else
+  (
+    assert (Usize.v h_index_new > heap_size); //h_index_new is greater than heap_size means the last object size exceeds the heap.
+    ()
+  )
+)
+
+let wosize_times_mword_multiple_of_mword5 (wz:wosize)
+                     :Lemma
+                      (ensures (Usize.v (Usize.mul (Usize.add wz 1UL)  mword) % Usize.v mword == 0)) = ()
 
 
-val objects2_equal_lemma3 :(h_index:hp_addr) ->
-                           (g:heap) ->
-                           (g':heap) ->
-                       Lemma
+
+
+
+
+let objects2_mem_lemma1_app3 (h_index: hp_addr)
+                            (g:heap)
+
+
+          : Lemma
+            (requires (Seq.length (objects2 0UL g) > 0 /\ Seq.mem h_index (objects2 0UL g) /\
+                        Usize.v (Usize.add h_index (Usize.mul (Usize.add (getWosize (read_word g h_index)) 1UL) mword)) < heap_size))
+            (ensures (Seq.mem (Usize.add h_index (Usize.mul (Usize.add (getWosize (read_word g h_index)) 1UL) mword)) (objects2 0UL g))) =
+
+  let s = objects2 0UL g in
+  objects2_mem_lemma1 0UL g;
+  let h_index_new = Usize.add h_index (Usize.mul (Usize.add (getWosize (read_word g h_index)) 1UL) mword) in
+  assert (Usize.v h_index_new < heap_size);
+  assert (Seq.mem h_index_new s);
+  ()
+
+#restart-solver
+
+#restart-solver
+
+
+
+let rec objects2_equal_lemma3  (h_index:hp_addr) 
+                           (g:heap) 
+                           (g':heap) 
+                      : Lemma
                        (requires (objects2 0UL g == objects2 0UL g') /\
                                  (Seq.mem h_index (objects2 0UL g)) /\
                                  (forall x. Seq.mem x (objects2 0UL g) ==> getWosize (read_word g x) == getWosize (read_word g' x)))
                        (ensures objects2 h_index g == objects2 h_index g')
-                       (decreases (heap_size - Usize.v h_index))
-                       
-val objects2_length_lemma :(h_index:hp_addr) ->
-                           (g:heap) ->
-                     Lemma
-                     (ensures (Seq.length (objects2 h_index g) <= (heap_size - Usize.v h_index)))
-                     (decreases (heap_size - Usize.v h_index))
+                       (decreases (heap_size - Usize.v h_index)) =
+  let wz =  getWosize (read_word g h_index) in
+let wz1 =  getWosize (read_word g' h_index) in
+assert (wz == wz1);
+if Usize.v wz = 0 then () // There are no zero length objects.
+else
+(
+  let h_index_new =  Usize.add h_index (Usize.mul (Usize.add wz 1UL) mword) in // possible next header = h_index + (wz + 1) * mword. Eg. h_index = 0; wz = 1; mword = 8;
+  wosize_times_mword_multiple_of_mword wz;
+  assert (Usize.v (Usize.mul (Usize.add wz 1UL) mword) % Usize.v mword == 0);
 
-val objects2_color_lemma : (h_index:hp_addr) ->
-                           (g:heap) ->
-                     Lemma
+  sum_of_multiple_of_mword_is_multiple_of_mword h_index (Usize.mul (Usize.add wz 1UL) mword);                                                                             // h_index_new = 0 +
+                                                                      // first field range in g = 8......15. Only one field. So next header starts at 16
+  assert ((Usize.v h_index + Usize.v (Usize.mul (Usize.add wz 1UL) mword)) % Usize.v mword == 0);
+  assert (Usize.v h_index_new % Usize.v mword == 0);
+  if Usize.v h_index_new <= heap_size then //valid heap condition
+  (
+    if Usize.v h_index_new = heap_size then // h_index_new == heap_size --> The last block is h_index, So just create a singleton with h_index and return.
+    (
+       assert (Usize.v h_index_new == heap_size);
+       let f = Seq.create 1 h_index in
+
+       G.is_vertex_set_lemma2 f;
+       ()
+    )
+    else
+    (
+      assert (Usize.v h_index_new < heap_size); // h_index_new < heap_size, still more blocks to explore, hence recurse.
+      assert (is_hp_addr h_index_new);
+      let f' =  objects2 h_index_new g in
+      objects2_mem_lemma1_app3 h_index g;
+      assert (Seq.mem h_index_new (objects2 0UL g));
+      objects2_equal_lemma3 h_index_new g g';
+      if length f' = 0 then ()
+       else
+       (
+         (*lemma_tail_snoc f' h_index;
+         lemma_mem_snoc f' h_index;
+         let f'' = snoc f' h_index in
+
+         G.snoc_unique_lemma h_index f';*)
+         assert (Seq.mem h_index (objects2 0UL g));
+         lemma_tl h_index f';
+         let f'' = cons h_index f' in
+         assert (Seq.length f'' > 0 /\ (Usize.v h_index_new < heap_size) ==> Seq.mem h_index_new f'');
+         G.is_vertex_set_cons h_index f';
+
+         ()
+       )
+    )
+  )
+  else
+  (
+    assert (Usize.v h_index_new > heap_size); //h_index_new is greater than heap_size means the last object size exceeds the heap.
+    ()
+  )
+)
+
+                   
+let rec objects2_length_lemma (h_index:hp_addr) 
+                           (g:heap)
+                    :Lemma
+                     (ensures (Seq.length (objects2 h_index g) <= (heap_size - Usize.v h_index)))
+                     (decreases (heap_size - Usize.v h_index)) =
+  
+let wz =  getWosize (read_word g h_index) in
+
+if Usize.v wz = 0 then () // There are no zero length objects.
+else
+(
+  let h_index_new =  Usize.add h_index (Usize.mul (Usize.add wz 1UL) mword) in // possible next header = h_index + (wz + 1) * mword. Eg. h_index = 0; wz = 1; mword = 8;
+                                                                               // h_index_new = 0 + (1 + 1) * 8 = 0 + 16 = 16. h_index range in g = 0......7
+                                                                               // first field range in g = 8......15. Only one field. So next header starts at 16
+  if Usize.v h_index_new <= heap_size then //valid heap condition
+  (
+    if Usize.v h_index_new = heap_size then // h_index_new == heap_size --> The last block is h_index, So just create a singleton with h_index and return.
+    (
+       assert (Usize.v h_index_new == heap_size);
+       let f = Seq.create 1 h_index in
+
+       G.is_vertex_set_lemma2 f;
+       ()
+    )
+    else
+    (
+      assert (Usize.v h_index_new < heap_size); // h_index_new < heap_size, still more blocks to explore, hence recurse.
+      let f' =  objects2 h_index_new g in
+      objects2_length_lemma h_index_new g;
+      if length f' = 0 then ()
+       else
+       (
+         (*lemma_tail_snoc f' h_index;
+         lemma_mem_snoc f' h_index;
+         let f'' = snoc f' h_index in
+
+         G.snoc_unique_lemma h_index f';*)
+         lemma_tl h_index f';
+         let f'' = cons h_index f' in
+         assert (Seq.length f'' > 0 /\ (Usize.v h_index_new < heap_size) ==> Seq.mem h_index_new f'');
+         G.is_vertex_set_cons h_index f';
+         ()
+       )
+    )
+  )
+  else
+  (
+    assert (Usize.v h_index_new > heap_size); //h_index_new is greater than heap_size means the last object size exceeds the heap.
+    ()
+  )
+)
+
+let rec objects2_color_lemma  (h_index:hp_addr) 
+                           (g:heap) 
+                    : Lemma
                      (ensures (forall x. Seq.mem x (objects2 h_index g) ==> color_of_object1 x g == white \/
                                                                        color_of_object1 x g == gray \/
                                                                        color_of_object1 x g == black \/
                                                                        color_of_object1 x g == blue))
-                     (decreases (heap_size - Usize.v h_index))
+                     (decreases (heap_size - Usize.v h_index)) =
+  let wz =  getWosize (read_word g h_index) in
+  color_lemma h_index g;
+if Usize.v wz = 0 then () // There are no zero length objects.
+else
+(
+  let h_index_new =  Usize.add h_index (Usize.mul (Usize.add wz 1UL) mword) in // possible next header = h_index + (wz + 1) * mword. Eg. h_index = 0; wz = 1; mword = 8;
+                                                                               // h_index_new = 0 + (1 + 1) * 8 = 0 + 16 = 16. h_index range in g = 0......7
+   wosize_times_mword_multiple_of_mword wz;
+  assert (Usize.v (Usize.mul wz mword) % Usize.v mword == 0);
 
+  sum_of_multiple_of_mword_is_multiple_of_mword h_index (Usize.mul wz mword);
+  if Usize.v h_index_new <= heap_size then //valid heap condition
 
+  (
+    if Usize.v h_index_new = heap_size then // h_index_new == heap_size --> The last block is h_index, So just create a singleton with h_index and return.
+    (
+       assert (Usize.v h_index_new == heap_size);
+       let f = Seq.create 1 h_index in
+
+       G.is_vertex_set_lemma2 f;
+       ()
+    )
+    else
+    (
+      assert (Usize.v h_index_new < heap_size); // h_index_new < heap_size, still more blocks to explore, hence recurse.
+      let f' =  objects2 h_index_new g in
+      objects2_color_lemma h_index_new g;
+      assert ((forall x. Seq.mem x (objects2 h_index_new g) ==> color_of_object1 x g == white \/
+                                                           color_of_object1 x g == gray \/
+                                                           color_of_object1 x g == black \/
+                                                           color_of_object1 x g == blue));
+      assert ((forall x. Seq.mem x f' ==> color_of_object1 x g == white \/
+                                     color_of_object1 x g == gray \/
+                                     color_of_object1 x g == black \/
+                                     color_of_object1 x g == blue));
+      assert (color_of_object1 h_index g == white \/
+              color_of_object1 h_index g == gray \/
+              color_of_object1 h_index g == black \/
+              color_of_object1 h_index g == blue);
+      if length f' = 0 then ()
+       else
+       (
+         (*lemma_tail_snoc f' h_index;
+         lemma_mem_snoc f' h_index;
+         let f'' = snoc f' h_index in
+
+         G.snoc_unique_lemma h_index f';*)
+         lemma_tl h_index f';
+         let f'' = cons h_index f' in
+         assert (Seq.length f'' > 0 /\ (Usize.v h_index_new < heap_size) ==> Seq.mem h_index_new f'');
+         G.is_vertex_set_cons h_index f';
+         ()
+       )
+    )
+  )
+  else
+  (
+    assert (Usize.v h_index_new > heap_size); //h_index_new is greater than heap_size means the last object size exceeds the heap.
+    ()
+  )
+)
+
+let rec get_allocs_helper (g:heap{Seq.length (objects2 0UL g) > 0})
+                          (f: seq Usize.t {(forall x. Seq.mem x f ==> Usize.v x >= 0 /\ Usize.v x < heap_size) /\
+                                           (forall x. Seq.mem x f ==> Usize.v x % Usize.v mword == 0) /\
+                                           (G.is_vertex_set f) /\
+                                           (forall x. Seq.mem x f ==> Seq.mem x (objects2 0UL g))})
+                    : Tot (allocs: seq Usize.t{(forall x. Seq.mem x allocs ==> Usize.v x >= 0 /\ Usize.v x < heap_size) /\
+                                               (forall x. Seq.mem x allocs ==> Usize.v x % Usize.v mword == 0) /\
+                                               (G.is_vertex_set allocs) /\
+                                               (forall x. Seq.mem x allocs ==> Seq.mem x f) /\
+                                               (G.subset_vertices allocs f) /\
+                                               (forall x. Seq.mem x allocs ==>
+                                                  Seq.mem x (objects2 0UL g)) /\
+                                               (forall x. Seq.mem x allocs ==> Seq.mem x (objects2 0UL g)) /\
+                                               (forall x. Seq.mem x allocs ==> (isWhiteObject1 x g) \/ (isGrayObject1 x g) \/
+                                                                        (isBlackObject1 x g)) /\
+                                               (forall x. Seq.mem x f /\
+                                                            ((isWhiteObject1 x g) \/ (isGrayObject1 x g) \/
+                                                                        (isBlackObject1 x g))==>
+                                                         Seq.mem x allocs) /\
+                                               (forall x. Seq.mem x f /\ (isWhiteObject1 x g) ==> Seq.mem x allocs) /\
+                                               (forall x. Seq.mem x f /\ (isBlackObject1 x g) ==> Seq.mem x allocs) /\
+                                               (forall x. Seq.mem x f /\ (isGrayObject1 x g) ==> Seq.mem x allocs)})
+                      (decreases length f) =
+if length f = 0 then
+(
+ G.is_vertex_set_lemma1 f;
+ assert (G.is_vertex_set f);
+ assert (G.subset_vertices f f);
+ assert (forall x. Seq.mem x f /\ (isWhiteObject1 x g) ==> Seq.mem x f);
+ f
+)
+else
+ (
+   let hd = Seq.head f in
+   let tl = Seq.tail f in
+
+   assert (forall x. Seq.mem x f ==> Usize.v x >= 0 /\ Usize.v x < heap_size);
+   assert (forall x. Seq.mem x tl ==> Usize.v x >= 0 /\ Usize.v x < heap_size);
+   assert (G.is_vertex_set f);
+
+   G.is_vertex_set_lemma f;
+   assert (G.is_vertex_set tl);
+
+   G.is_vertex_set_lemma4 f;
+   assert (~(Seq.mem hd tl));
+
+   let allocs' = get_allocs_helper g tl in
+   assert (forall x. Seq.mem x tl /\ (isWhiteObject1 x g) ==> Seq.mem x allocs');
+   assert (forall x. Seq.mem x allocs' ==> Seq.mem x tl);
+   assert (~(Seq.mem hd allocs'));
+   assert (Seq.mem hd f);
+   objects2_color_lemma 0UL g;
+   assert (forall x. Seq.mem x (objects2 0UL g) ==> color_of_object1 x g == white \/
+                                               color_of_object1 x g == gray \/
+                                               color_of_object1 x g == black \/
+                                               color_of_object1 x g == blue);
+   assert (forall x. Seq.mem x f ==> Seq.mem x (objects2 0UL g));
+   assert (color_of_object1 hd g == white \/ color_of_object1 hd g == gray \/ color_of_object1 hd g == black \/ color_of_object1 hd g == blue);
+   if (isWhiteObject1 hd g || isGrayObject1 hd g || isBlackObject1 hd g) then
+     (
+       if length allocs' > 0 then
+       (
+          Seq.lemma_tail_snoc allocs' hd;
+          Seq.lemma_mem_snoc allocs' hd;
+          let allocs'' = snoc allocs' hd in
+          assert (G.is_vertex_set allocs');
+          assert (~(Seq.mem hd allocs'));
+          G.snoc_unique_lemma hd allocs';
+          assert (G.is_vertex_set allocs'');
+          assert (G.subset_vertices allocs'' f);
+          allocs''
+
+       )
+       else
+       (
+         let allocs'' =  Seq.cons hd (Seq.empty) in//Seq.create 1 hd in
+         lemma_tl hd (Seq.empty);
+         G.is_vertex_set_lemma2 allocs'';
+         assert (Seq.mem hd f);
+         assert (Seq.length allocs'' == 1);
+         assert (Seq.head allocs'' == hd);
+         assert (Seq.tail allocs'' == Seq.empty);
+         lemma_mem_inversion allocs'';
+         assert (forall x. mem x allocs'' = (x = head allocs'' || mem x (tail allocs'')));
+         assert (forall x. mem x allocs'' ==> (x = head allocs'' || mem x (tail allocs'')));
+         assert (forall x. mem x allocs'' ==> (x = hd || mem x (Seq.empty)));
+         assert (forall x. mem x allocs'' ==> (x = hd));
+         assert (forall x. mem x allocs'' ==> Seq.mem x f);
+         assert (forall x. Seq.mem x allocs'' ==> Seq.mem x f);
+         assert (G.subset_vertices allocs'' f);
+         allocs''
+       )
+
+     )
+   else
+     (
+      assert (forall x. Seq.mem x allocs' ==> Seq.mem x tl);
+      assert (forall x. Seq.mem x allocs' ==> Seq.mem x f);
+      assert (G.subset_vertices allocs' f);
+      allocs'
+     )
+  )
 
 #restart-solver
 
@@ -682,9 +1481,178 @@ let heap_remains_same_except_index_v_id  (v_id:hp_addr)
   forall (x:Usize.t {Usize.v x < heap_size /\ (Usize.v x % Usize.v mword == 0)}). x <> v_id ==>
            read_word g x == read_word g' x 
            
+let snoc_equality_lemma (f: seq Usize.t{Seq.length f > 0})
+                        (f': seq Usize.t{Seq.length f' > 0})
+                        (hd: Usize.t)
+                        (hd': Usize.t)
+                : Lemma
+                  (requires f == f' /\ hd == hd')
+                  (ensures (snoc f hd == snoc f' hd')) = ()
 
-val get_allocated_block_addresses  : (g:heap {Seq.length (objects2 0UL g) > 0}) ->
-                           Tot (allocs: seq Usize.t {(forall x. Seq.mem x allocs ==> Usize.v x >= 0 /\ Usize.v x < heap_size) /\
+#restart-solver
+
+#restart-solver
+
+#restart-solver
+
+let seq_mem_lemma (f: seq Usize.t{Seq.length f > 0})
+            : Lemma
+              (ensures(Seq.mem (Seq.head f) f) /\
+                      (forall x. Seq.mem x (Seq.tail f) ==> Seq.mem x f)) = ()
+
+let seq_length_tl_lemma (f: seq Usize.t{Seq.length f > 0})
+            : Lemma
+              (ensures (Seq.length (Seq.tail f) < Seq.length f)) = ()
+
+
+let seq_empty_length_lemma ()
+            : Lemma
+              (ensures (Seq.length (Seq.empty) == 0)) = ()
+
+let seq_cons_length_mem_lemma (hd:Usize.t)
+                   : Lemma
+                     (ensures (Seq.length (Seq.cons hd (Seq.empty)) == 1) /\
+                              (Seq.head (Seq.cons hd (Seq.empty)) == hd) /\
+                              (Seq.tail (Seq.cons hd (Seq.empty)) == Seq.empty)) = ()
+
+let seq_empty_mem_lemma (#a:eqtype)
+            : Lemma
+              (ensures ~(exists x.Seq.mem x (Seq.empty #a))) = ()
+
+
+#reset-options "--z3rlimit 50  --max_fuel 1 --max_ifuel 1 --using_facts_from '* -FStar.Seq'"
+
+#push-options "--split_queries always"
+
+#restart-solver
+let rec get_allocs_helper_lemma (g:heap{Seq.length (objects2 0UL g) > 0})
+                                (g':heap{Seq.length (objects2 0UL g') > 0})
+                                (f: seq Usize.t {(forall x. Seq.mem x f ==> Usize.v x >= 0 /\ Usize.v x < heap_size) /\
+                                                 (forall x. Seq.mem x f ==> Usize.v x % Usize.v mword == 0) /\
+                                                 (G.is_vertex_set f) /\
+                                                 (forall x. Seq.mem x f ==> is_hp_addr x) /\
+                                                 (forall x. Seq.mem x f ==> Seq.mem x (objects2 0UL g))})
+                                (f': seq Usize.t {(forall x. Seq.mem x f' ==> Usize.v x >= 0 /\ Usize.v x < heap_size) /\
+                                                  (forall x. Seq.mem x f' ==> Usize.v x % Usize.v mword == 0) /\
+                                                  (G.is_vertex_set f') /\
+                                                  (forall x. Seq.mem x f' ==> is_hp_addr x) /\
+                                                  (forall x. Seq.mem x f' ==> Seq.mem x (objects2 0UL g'))})
+                                (v_id:hp_addr)
+                                (c:color)
+                      : Lemma
+                        (requires (objects2 0UL g ==
+                                   objects2 0UL g') /\
+                                  (f == f') /\
+                                  (Seq.length g == Seq.length g') /\
+                                  (heap_remains_same_except_index_v_id v_id g g') /\
+                                  (color_of_object1 v_id g' == c) /\
+                                  (color_of_object1 v_id g == white \/ color_of_object1 v_id g == gray \/
+                                    color_of_object1 v_id g == black) /\
+                                  (wosize_of_object1 v_id g' == wosize_of_object1 v_id g) /\
+                                  (tag_of_object1 v_id g' == tag_of_object1 v_id g) /\
+                                  (Seq.mem v_id (objects2 0UL g)) /\
+                                  (Seq.mem v_id (objects2 0UL g')) /\
+                                  (c == 1UL \/ c == 2UL \/ c == 3UL))
+                         (ensures (get_allocs_helper g f == get_allocs_helper g' f'))
+                         (decreases (Seq.length f))=
+if length f = 0 then
+  (
+     G.is_vertex_set_lemma1 f;
+     assert (G.is_vertex_set f);
+     assert (G.subset_vertices f f);
+     assert (get_allocs_helper g f == get_allocs_helper g' f');
+     ()
+)
+else
+ (
+   let hd = Seq.head f in
+   let tl = Seq.tail f in
+
+   let hd' = Seq.head f' in
+   let tl' = Seq.tail f' in
+
+   assert (hd == hd');
+   assert (tl == tl');
+
+   G.is_vertex_set_lemma f;
+   G.is_vertex_set_lemma f';
+
+   assert (G.is_vertex_set f /\ length f > 0 ==> G.is_vertex_set (tail f));
+   assert (G.is_vertex_set (tail f));
+   assert (tl == tail f);
+   assert (G.is_vertex_set tl);
+   assert (G.is_vertex_set tl');
+
+   G.is_vertex_set_lemma4 f;
+   G.is_vertex_set_lemma4 f';
+   seq_mem_lemma f;
+   let allocs' = get_allocs_helper g tl in
+   let allocs'' = get_allocs_helper g' tl' in
+
+   seq_length_tl_lemma f;
+   get_allocs_helper_lemma g g' tl tl' v_id c;
+
+   //assert (G.is_vertex_set tl);
+   assert (get_allocs_helper g tl == get_allocs_helper g' tl');
+
+   if (isWhiteObject1 hd g || isGrayObject1 hd g || isBlackObject1 hd g) then
+     (
+       assert (isWhiteObject1 hd g || isGrayObject1 hd g || isBlackObject1 hd g);
+       assert (isWhiteObject1 hd g' || isGrayObject1 hd g' || isBlackObject1 hd g');
+       if length allocs' > 0 then
+       (
+          Seq.lemma_tail_snoc allocs' hd;
+          Seq.lemma_mem_snoc allocs' hd;
+          Seq.lemma_tail_snoc allocs'' hd';
+          Seq.lemma_mem_snoc allocs'' hd';
+          let allocs1 = snoc allocs' hd in
+          let allocs2 = snoc allocs'' hd' in
+
+          G.snoc_unique_lemma hd allocs';
+          G.snoc_unique_lemma hd' allocs'';
+          assert (allocs'' == allocs');
+          assert (hd == hd');
+          snoc_equality_lemma allocs' allocs'' hd hd';
+          assert (allocs1 == allocs2);
+          ()
+       )
+       else
+       (
+         let allocs1 =  Seq.cons hd (Seq.empty) in//Seq.create 1 hd in
+         seq_empty_length_lemma #UInt64.t ();
+         lemma_tl hd (Seq.empty);
+         G.is_vertex_set_lemma2 allocs1;
+         assert (Seq.mem hd f);
+         seq_cons_length_mem_lemma hd;
+         assert (Seq.length allocs1 == 1);
+         assert (Seq.head allocs1 == hd);
+         assert (Seq.tail allocs1 == Seq.empty);
+         lemma_mem_inversion allocs1;
+         assert (forall x. mem x allocs1 = (x = head allocs1 || mem x (tail allocs1)));
+         assert (forall x. mem x allocs1 ==> (x = head allocs1 || mem x (tail allocs1)));
+         assert (forall x. mem x allocs1 ==> (x = hd || mem x (Seq.empty)));
+         seq_empty_mem_lemma #UInt64.t;
+         assert (forall x. mem x allocs1 ==> (x = hd));
+         assert (forall x. mem x allocs1 ==> Seq.mem x f);
+         assert (forall x. Seq.mem x allocs1 ==> Seq.mem x f);
+         assert (G.subset_vertices allocs1 f);
+         ()
+
+       )
+     )
+   else
+     (
+        ()
+     )
+ )
+
+#reset-options "--z3rlimit 500"
+
+#push-options "--split_queries always"
+
+
+let get_allocated_block_addresses   (g:heap {Seq.length (objects2 0UL g) > 0}) 
+                           :Tot (allocs: seq Usize.t {(forall x. Seq.mem x allocs ==> Usize.v x >= 0 /\ Usize.v x < heap_size) /\
                                                       (forall x. Seq.mem x allocs ==> is_hp_addr x) /\
                                                       (forall x. Seq.mem x allocs ==> Seq.mem x (objects2 0UL g)) /\
                                                       (G.is_vertex_set allocs) /\
@@ -694,16 +1662,48 @@ val get_allocated_block_addresses  : (g:heap {Seq.length (objects2 0UL g) > 0}) 
                                                                                 (isBlackObject1 x g)) /\
                                                       (forall x. Seq.mem x (objects2 0UL g) /\
                                                            ((isWhiteObject1 x g) \/ (isGrayObject1 x g) \/ (isBlackObject1 x g))==>
-                                                               Seq.mem x allocs)})
+                                                               Seq.mem x allocs)}) =
+  
+ let f =  objects2 0UL g in
+   assert (length f > 0);
+   assert (forall x. Seq.mem x f ==> Usize.v x >= 0 /\ Usize.v x < heap_size);
+   assert (G.is_vertex_set f);
+   assert (forall x. Seq.mem x f ==> Usize.v x >= 0);
+
+   let allocs = get_allocs_helper g f in
+   assert (G.is_vertex_set allocs);
+   assert (G.subset_vertices allocs f);
+   assert (G.subset_vertices allocs (objects2 0UL g));
+   assert (forall x. Seq.mem x allocs ==> (isWhiteObject1 x g) \/ (isGrayObject1 x g) \/ (isBlackObject1 x g));
+   assert (forall x. Seq.mem x f /\ ((isWhiteObject1 x g) \/ (isGrayObject1 x g) \/ (isBlackObject1 x g))==>
+                                                     Seq.mem x allocs);
+   assert (forall x. Seq.mem x (objects2 0UL g) /\
+                          ((isWhiteObject1 x g) \/ (isGrayObject1 x g) \/ (isBlackObject1 x g))==>
+                                                     Seq.mem x allocs);
+   assert (forall x. Seq.mem x f /\ (isWhiteObject1 x g) ==> Seq.mem x allocs);
+   assert (forall x. Seq.mem x f /\ (isBlackObject1 x g) ==> Seq.mem x allocs);
+   assert (forall x. Seq.mem x f /\ (isGrayObject1 x g) ==> Seq.mem x allocs);
+   allocs
+
+let cons_lemma_mem (hd:Usize.t)
+                       (l: seq Usize.t)
+                       (f: seq Usize.t)
+               : Lemma
+                 (requires (G.is_vertex_set l) /\ (G.is_vertex_set f) /\ ~(Seq.mem hd l) /\ (Seq.mem hd f) /\ (G.subset_vertices l f))
+                 (ensures (forall x. Seq.mem x (Seq.cons hd l) ==> Seq.mem x f)) =
+ let l1 = Seq.cons hd l in
+ Seq.lemma_tl hd l;
+ Seq.mem_cons hd l;
+ ()
 
 
-val is_fields_contents_within_limit2_lemma_for_sweep :  (h_index: hp_addr) ->
-                                                           (wz: wosize{is_fields_within_limit1 h_index wz}) ->
-                                                           (wz': wosize{is_fields_within_limit1 h_index wz'})->
-                                                           (g:heap{Seq.length (objects2 0UL g) > 0}) ->
-                                                           (g':heap{Seq.length (objects2 0UL g') > 0})->
+let rec is_fields_contents_within_limit2_lemma_for_sweep   (h_index: hp_addr) 
+                                                           (wz: wosize{is_fields_within_limit1 h_index wz}) 
+                                                           (wz': wosize{is_fields_within_limit1 h_index wz'})
+                                                           (g:heap{Seq.length (objects2 0UL g) > 0}) 
+                                                           (g':heap{Seq.length (objects2 0UL g') > 0})
                                           
-                          Lemma
+                         : Lemma
                             (requires (wz == wz') /\
                                       (Seq.mem h_index (get_allocated_block_addresses g) /\
                                        Seq.mem h_index (get_allocated_block_addresses g')) /\
@@ -717,19 +1717,145 @@ val is_fields_contents_within_limit2_lemma_for_sweep :  (h_index: hp_addr) ->
                                                                  
                             (ensures (*(is_fields_contents_within_limit2 h_index wz g == true <==>*)
                                       is_fields_contents_within_limit2 h_index wz' g' == true)
-                            (decreases (Usize.v wz))
+                            (decreases (Usize.v wz)) =
+  if (Usize.v wz = 0) then ()
+ else
+ (
+  assert (Usize.v wz > 0);
+   let s = Usize.add h_index (Usize.mul wz mword) in
+   let wz1 = Usize.sub wz 1UL in
+   let wz2 = Usize.sub wz' 1UL in
+    wosize_times_mword_multiple_of_mword wz;
+    assert (Usize.v (Usize.mul wz mword) % Usize.v mword == 0);
+
+    sum_of_multiple_of_mword_is_multiple_of_mword h_index (Usize.mul wz mword);
+    assert (is_hp_addr s);
+    let succ = read_word g s in
+    let succ' = read_word g' s in
+    assert (succ == succ');
+    if (isPointer s g) then
+   (
+
+     if Usize.v succ >= Usize.v mword && Usize.v succ < heap_size && is_hp_addr succ then
+         is_fields_contents_within_limit2_lemma_for_sweep h_index wz1 wz2 g g'
+
+     else
+         ()
+   )
+   else
+   (
+     assert (~(isPointer s g));
+      is_fields_contents_within_limit2_lemma_for_sweep h_index wz1 wz2 g g';
+     ()
+   )
+ )
+
+let rec get_color_based_block_picker (g:heap{Seq.length (objects2 0UL g) > 0})
+                                     (f: seq Usize.t {(forall x. Seq.mem x f ==> Usize.v x >= 0 /\ Usize.v x < heap_size) /\
+                                                      (forall x. Seq.mem x f ==> Usize.v x % Usize.v mword == 0) /\
+                                                      (G.is_vertex_set f) /\
+                                                      (G.subset_vertices f (objects2 0UL g)) /\
+                                                      (forall x. Seq.mem x f ==> Seq.mem x (objects2 0UL g)) /\
+                                                      (forall x. Seq.mem x f ==> (isWhiteObject1 x g) \/
+                                                                            (isGrayObject1 x g) \/
+                                                                            (isBlackObject1 x g))})
+
+                                     (c:color{c == white \/ c == gray \/ c == black})
+
+                    : Tot (color_block: seq Usize.t{(forall x. Seq.mem x color_block ==> Usize.v x >= 0 /\ Usize.v x < heap_size)  /\
+                                                    (forall x. Seq.mem x color_block ==> Usize.v x % Usize.v mword == 0) /\
+                                                    (G.is_vertex_set color_block) /\
+                                                    (forall x. Seq.mem x color_block ==> Seq.mem x f) /\
+                                                    (G.subset_vertices color_block f) /\
+                                                    (G.subset_vertices color_block (objects2 0UL g)) /\
+                                                    (forall x. Seq.mem x color_block ==>  Seq.mem x (objects2 0UL g)) /\
+                                                    (forall x. Seq.mem x color_block ==> Seq.mem x f /\ color_of_object1 x g == c) /\
+                                                    (forall x. Seq.mem x f /\ color_of_object1 x g == c ==> Seq.mem x color_block) /\
+                                                    (forall x. Seq.mem x color_block <==> Seq.mem x f /\ color_of_object1 x g == c)})
+
+                      (decreases length f) =
+assert (forall x. Seq.mem x f ==>  color_of_object1 x g == black \/
+                             color_of_object1 x g == white \/
+                             color_of_object1 x g == gray);
+if length f = 0 then
+(
+ G.is_vertex_set_lemma1 f;
+ assert (G.is_vertex_set f);
+ assert (G.subset_vertices f f);
+ assert (G.subset_vertices f (objects2 0UL g));
+ assert (forall x. Seq.mem x f ==> Seq.mem x f /\ color_of_object1 x g == c);
+ assert (forall x. Seq.mem x f <==> Seq.mem x f /\ color_of_object1 x g == c);
+ f
+)
+else
+ (
+    let hd = Seq.head f in
+    let tl = Seq.tail f in
+
+    G.is_vertex_set_lemma f;
+
+    G.is_vertex_set_lemma4 f;
+
+    let color_block' = get_color_based_block_picker g tl c in
+    assert (forall x. Seq.mem x color_block' ==> Seq.mem x tl);
+    assert (~(Seq.mem hd color_block'));
+    if (color_of_object1 hd g = c) then
+     (
+        if length color_block' > 0 then
+          (
+             Seq.lemma_tail_snoc color_block' hd;
+             Seq.lemma_mem_snoc color_block' hd;
+             let color_block'' = snoc color_block' hd in
+             assert (G.is_vertex_set color_block');
+             assert (~(Seq.mem hd color_block'));
+             G.snoc_unique_lemma hd color_block';
+             assert (G.is_vertex_set color_block'');
+             assert (G.subset_vertices color_block'' f);
+             assert (forall x. Seq.mem x color_block'' ==> Seq.mem x f /\ color_of_object1 x g == c);
+             assert (forall x. Seq.mem x color_block'' <==> Seq.mem x f /\ color_of_object1 x g == c);
+             color_block''
+          )
+        else
+          (
+             Seq.lemma_tl hd color_block';
+             let color_block'' = Seq.cons hd color_block' in
+             assert (~(Seq.mem hd color_block'));
+             G.is_vertex_set_cons hd color_block';
+             assert (G.is_vertex_set color_block'');
+             assert (forall x. Seq.mem x color_block' ==> Seq.mem x f);
+             assert (Seq.mem hd f);
+             Seq.mem_cons hd color_block';
+             assert (forall x. Seq.mem x color_block'' ==> Seq.mem x f);
+             assert (G.subset_vertices color_block'' f);
+             assert (G.subset_vertices color_block'' (objects2 0UL g));
+             assert (forall x. Seq.mem x color_block'' ==> Seq.mem x f /\ color_of_object1 x g == c);
+             assert (forall x. Seq.mem x color_block'' <==> Seq.mem x f /\ color_of_object1 x g == c);
+             color_block''
+          )
+     )
+
+    else
+     (
+        assert (G.is_vertex_set color_block');
+        assert (G.subset_vertices color_block' f);
+        assert (G.subset_vertices color_block' (objects2 0UL g));
+        assert (forall x. Seq.mem x color_block' ==> Seq.mem x f /\ color_of_object1 x g == c);
+        assert (forall x. Seq.mem x color_block' <==> Seq.mem x f /\ color_of_object1 x g == c);
+        color_block'
+     )
+ )
+
 
 #restart-solver
 
-//#reset-options "--z3rlimit 50 --max_fuel 0 --max_ifuel 0 --using_facts_from '* -FStar.Seq'"
+#reset-options "--z3rlimit 50"
 
-#restart-solver
 
-val get_allocated_block_addresses_lemma :   (g:heap {Seq.length (objects2 0UL g) > 0}) ->
-                                            (g':heap{Seq.length (objects2 0UL g') > 0})->
-                                            (v_id:hp_addr) ->
-                                            (c:color)->
-                           Lemma
+let get_allocated_block_addresses_lemma     (g:heap {Seq.length (objects2 0UL g) > 0}) 
+                                            (g':heap{Seq.length (objects2 0UL g') > 0})
+                                            (v_id:hp_addr) 
+                                            (c:color)
+                          : Lemma
                            (requires (objects2 0UL g ==
                                       objects2 0UL g') /\
                                       Seq.length g == Seq.length g' /\
@@ -741,13 +1867,24 @@ val get_allocated_block_addresses_lemma :   (g:heap {Seq.length (objects2 0UL g)
                                       tag_of_object1 v_id g' == tag_of_object1 v_id g /\
                                       Seq.mem v_id (objects2 0UL g) /\ Seq.mem v_id (objects2 0UL g') /\
                                       (c == 1UL \/ c == 2UL \/ c == 3UL))
-                           (ensures (get_allocated_block_addresses g == get_allocated_block_addresses g'))
+                           (ensures (get_allocated_block_addresses g == get_allocated_block_addresses g')) =
+  assert (length (objects2 0uL g) > 0);
+  let f =  objects2 0UL g in
+  let f' = objects2 0UL g' in
+  assert (length f > 0);
+  assert (f == f');
+  assert (length f > 0 ==> G.is_vertex_set f);
+  let allocs1 = get_allocs_helper g f in
+  let allocs2 = get_allocs_helper g' f' in
+  get_allocs_helper_lemma g g' f f' v_id c;
+  assert (allocs1 == allocs2);
+  assert (get_allocated_block_addresses g == get_allocated_block_addresses g');
+  ()
+
 
 #reset-options "--z3rlimit 500"
 
-
-
-val get_black_block_addresses : (g:heap {Seq.length (objects2 0UL g) > 0}) ->
+let get_black_block_addresses   (g:heap {Seq.length (objects2 0UL g) > 0}) 
                                 (allocs: seq Usize.t {Seq.equal allocs (get_allocated_block_addresses g) /\
                                                      (forall x. Seq.mem x allocs ==> Usize.v x >= 0 /\ Usize.v x < heap_size) /\
                                                      (forall x. Seq.mem x allocs ==> Usize.v x % Usize.v mword == 0) /\
@@ -757,8 +1894,8 @@ val get_black_block_addresses : (g:heap {Seq.length (objects2 0UL g) > 0}) ->
                                                        (objects2 0UL g)) /\
                                                      (forall x. Seq.mem x allocs ==> (isWhiteObject1 x g) \/ 
                                                                                (isGrayObject1 x g) \/
-                                                                               (isBlackObject1 x g))}) ->
-                            Tot (blacks: G.vertex_list (*seq Usize.t*)
+                                                                               (isBlackObject1 x g))}) 
+                           : Tot (blacks: G.vertex_list (*seq Usize.t*)
                                           {(forall x. Seq.mem x blacks ==> Usize.v x >= 0 /\ Usize.v x < heap_size) /\
                                                      (forall x. Seq.mem x blacks ==> Usize.v x % Usize.v mword == 0) /\
                                                      (forall x. Seq.mem x blacks ==> Seq.mem x (objects2 0UL g)) /\
@@ -774,10 +1911,32 @@ val get_black_block_addresses : (g:heap {Seq.length (objects2 0UL g) > 0}) ->
                                                          Seq.mem x (objects2 0UL g) /\
                                                          isBlackObject1 x g) /\
                                                      (forall x. Seq.mem x blacks <==> Seq.mem x (get_allocated_block_addresses g) /\ 
-                                                        color_of_object1 x g == black)})
+                                                        color_of_object1 x g == black)}) =
+ let blacks =  get_color_based_block_picker g allocs black in
+ assert (Seq.equal allocs (get_allocated_block_addresses g));
+ assert ((forall x. Seq.mem x allocs ==> (isWhiteObject1 x g) \/ (isGrayObject1 x g) \/ (isBlackObject1 x g)) /\
+         (forall x. Seq.mem x (objects2 0UL g) /\
+                               ((isWhiteObject1 x g) \/ (isGrayObject1 x g) \/ (isBlackObject1 x g))==>
+                                                      Seq.mem x allocs));
+ assert (forall x. Seq.mem x allocs /\ color_of_object1 x g == black ==> Seq.mem x blacks);
+ assert (forall x. Seq.mem x (objects2 0UL g) /\ isBlackObject1 x g ==>
+                                                      Seq.mem x blacks);
+ assert (forall x. Seq.mem x blacks ==> Seq.mem x (objects2 0UL g) /\ isBlackObject1 x g);
+ assert (forall x. Seq.mem x blacks <==> Seq.mem x (objects2 0UL g) /\ isBlackObject1 x g);
+ assert (forall x. Seq.mem x blacks ==> Usize.v x >= 0 /\ Usize.v x < heap_size);
+ assert (G.is_vertex_set blacks);
+ assert (forall x. Seq.mem x blacks ==> Seq.mem x allocs);
+ assert (G.subset_vertices blacks allocs /\
+        (G.subset_vertices blacks (objects2 0UL g)));
+ assert (forall x. Seq.mem x blacks ==> color_of_object1 x g == black);
+ assert (forall x. Seq.mem x blacks <==> Seq.mem x allocs /\ color_of_object1 x g == black);
+ assert (Seq.equal allocs (get_allocated_block_addresses g));
+ assert (forall x. Seq.mem x blacks <==> Seq.mem x (get_allocated_block_addresses g) /\ color_of_object1 x g == black);
+ blacks
 
-val get_gray_block_addresses : (g:heap {Seq.length (objects2 0UL g) > 0}) ->
-                                (allocs: seq Usize.t {Seq.equal allocs (get_allocated_block_addresses g) /\
+
+let get_gray_block_addresses   (g:heap {Seq.length (objects2 0UL g) > 0}) 
+                               (allocs: seq Usize.t {Seq.equal allocs (get_allocated_block_addresses g) /\
                                                    (forall x. Seq.mem x allocs ==> Usize.v x >= 0 /\ Usize.v x < heap_size) /\
                                                    (forall x. Seq.mem x allocs ==> Usize.v x % Usize.v mword == 0) /\
                                                    (forall x. Seq.mem x allocs ==> Seq.mem x (objects2 0UL g)) /\
@@ -786,8 +1945,8 @@ val get_gray_block_addresses : (g:heap {Seq.length (objects2 0UL g) > 0}) ->
                                                        (objects2 0UL g)) /\
                                                     (forall x. Seq.mem x allocs ==> (isWhiteObject1 x g) \/ 
                                                                                (isGrayObject1 x g) \/
-                                                                               (isBlackObject1 x g))}) ->
-                            Tot (grays: G.vertex_list (*seq Usize.t*)
+                                                                               (isBlackObject1 x g))}) 
+                           : Tot (grays: G.vertex_list (*seq Usize.t*)
                                           {(forall x. Seq.mem x grays ==> Usize.v x >= 0 /\ Usize.v x < heap_size) /\
                                                      (forall x. Seq.mem x grays ==> Usize.v x % Usize.v mword == 0) /\
                                                      (forall x. Seq.mem x grays ==> Seq.mem x (objects2 0UL g)) /\
@@ -803,9 +1962,32 @@ val get_gray_block_addresses : (g:heap {Seq.length (objects2 0UL g) > 0}) ->
                                                          Seq.mem x (objects2 0UL g) /\
                                                          isGrayObject1 x g) /\
                                                      (forall x. Seq.mem x grays <==> Seq.mem x (get_allocated_block_addresses g) /\ 
-                                                        color_of_object1 x g == gray)})
+                                                        color_of_object1 x g == gray)}) =
+ let grays =  get_color_based_block_picker g allocs 2UL in
+ assert (Seq.equal allocs (get_allocated_block_addresses g));
+ assert ((forall x. Seq.mem x allocs ==> (isWhiteObject1 x g) \/ (isGrayObject1 x g) \/ (isBlackObject1 x g)) /\
+         (forall x. Seq.mem x (objects2 0UL g) /\
+                               ((isWhiteObject1 x g) \/ (isGrayObject1 x g) \/ (isBlackObject1 x g))==>
+                                                      Seq.mem x allocs));
+ assert (forall x. Seq.mem x allocs /\ color_of_object1 x g == gray ==> Seq.mem x grays);
+ assert (forall x. Seq.mem x (objects2 0UL g) /\ isGrayObject1 x g ==>
+                                                      Seq.mem x grays);
+ assert (forall x. Seq.mem x grays ==> Seq.mem x (objects2 0UL g) /\ isGrayObject1 x g);
+ assert (forall x. Seq.mem x grays <==>
+   Seq.mem x (objects2 0UL g) /\ isGrayObject1 x g);
+ assert (forall x. Seq.mem x grays ==> Usize.v x >= 0 /\ Usize.v x < heap_size);
+ assert (G.is_vertex_set grays);
+ assert (forall x. Seq.mem x grays ==> Seq.mem x allocs);
+ assert (G.subset_vertices grays allocs /\
+          (G.subset_vertices  grays (objects2 0UL g)));
+ assert (forall x. Seq.mem x grays ==> color_of_object1 x g == gray);
+ assert (forall x. Seq.mem x grays <==> Seq.mem x allocs /\ color_of_object1 x g == gray);
+ assert (Seq.equal allocs (get_allocated_block_addresses g));
+ assert (forall x. Seq.mem x grays <==> Seq.mem x (get_allocated_block_addresses g) /\ color_of_object1 x g == gray);
+ grays
 
-val get_white_block_addresses : (g:heap {Seq.length (objects2 0UL g) > 0}) ->
+
+let get_white_block_addresses   (g:heap {Seq.length (objects2 0UL g) > 0}) 
                                 (allocs: seq Usize.t {Seq.equal allocs (get_allocated_block_addresses g) /\
                                                    (forall x. Seq.mem x allocs ==> Usize.v x >= 0 /\ Usize.v x < heap_size) /\
                                                    (forall x. Seq.mem x allocs ==> Usize.v x % Usize.v mword == 0) /\
@@ -815,8 +1997,8 @@ val get_white_block_addresses : (g:heap {Seq.length (objects2 0UL g) > 0}) ->
                                                        (objects2 0UL g)) /\
                                                     (forall x. Seq.mem x allocs ==> (isWhiteObject1 x g) \/ 
                                                                                (isGrayObject1 x g) \/
-                                                                               (isBlackObject1 x g))}) ->
-                            Tot (whites: G.vertex_list (*seq Usize.t*)
+                                                                               (isBlackObject1 x g))}) 
+                           : Tot (whites: G.vertex_list (*seq Usize.t*)
                                           {(forall x. Seq.mem x whites ==> Usize.v x >= 0 /\ Usize.v x < heap_size) /\
                                                      (forall x. Seq.mem x whites ==> Usize.v x % Usize.v mword == 0) /\
                                                      (forall x. Seq.mem x whites ==> Seq.mem x (objects2 0UL g)) /\
@@ -832,7 +2014,29 @@ val get_white_block_addresses : (g:heap {Seq.length (objects2 0UL g) > 0}) ->
                                                          Seq.mem x (objects2 0UL g) /\
                                                          isWhiteObject1 x g) /\
                                                      (forall x. Seq.mem x whites <==> Seq.mem x (get_allocated_block_addresses g) /\ 
-                                                        color_of_object1 x g == white)})
+                                                        color_of_object1 x g == white)}) =
+ let whites =  get_color_based_block_picker g allocs white in
+ assert (Seq.equal allocs (get_allocated_block_addresses g));
+ assert ((forall x. Seq.mem x allocs ==> (isWhiteObject1 x g) \/ (isGrayObject1 x g) \/ (isBlackObject1 x g)) /\
+         (forall x. Seq.mem x (objects2 0UL g) /\
+                               ((isWhiteObject1 x g) \/ (isGrayObject1 x g) \/ (isBlackObject1 x g))==>
+                                                      Seq.mem x allocs));
+ assert (forall x. Seq.mem x allocs /\ color_of_object1 x g == white ==> Seq.mem x whites);
+ assert (forall x. Seq.mem x (objects2 0UL g) /\ isWhiteObject1 x g ==>
+                                                      Seq.mem x whites);
+ assert (forall x. Seq.mem x whites ==> Seq.mem x (objects2 0UL g) /\ isWhiteObject1 x g);
+ assert (forall x. Seq.mem x whites <==>
+   Seq.mem x (objects2 0UL g) /\ isWhiteObject1 x g);
+ assert (forall x. Seq.mem x whites ==> Usize.v x >= 0 /\ Usize.v x < heap_size);
+ assert (G.is_vertex_set whites);
+ assert (forall x. Seq.mem x whites ==> Seq.mem x allocs);
+ assert (G.subset_vertices whites allocs /\
+          (G.subset_vertices whites (objects2 0UL g)));
+ assert (forall x. Seq.mem x whites ==> color_of_object1 x g == white);
+ assert (forall x. Seq.mem x whites <==> Seq.mem x allocs /\ color_of_object1 x g == white);
+ assert (Seq.equal allocs (get_allocated_block_addresses g));
+ assert (forall x. Seq.mem x whites <==> Seq.mem x (get_allocated_block_addresses g) /\ color_of_object1 x g == white);
+ whites
 
 #restart-solver 
 
@@ -1003,13 +2207,16 @@ let  condition_check_for_different_objects  (h_index: hp_addr{Usize.v h_index + 
                                                            fields_points_to_blocks_condition h_index g wz start_env_plus_one)
                                                          
                                                        ))
-val is_fields_contents_within_limit2_lemma : (h_index: hp_addr) ->
-                                             (wz: wosize{is_fields_within_limit1 h_index wz}) ->
-                                             (wz': wosize{is_fields_within_limit1 h_index wz'})->
-                                             (g:heap) ->
-                                             (g':heap) ->
+
+#restart-solver
+
+let rec is_fields_contents_within_limit2_lemma  (h_index: hp_addr) 
+                                                (wz: wosize{is_fields_within_limit1 h_index wz}) 
+                                                (wz': wosize{is_fields_within_limit1 h_index wz'})
+                                                (g:heap) 
+                                                (g':heap) 
                                           
-                            Lemma
+                           : Lemma
                             (requires (wz == wz') /\
                                       (forall (i:Usize.t {Usize.v i > 0 /\ Usize.v i <= Usize.v wz}). 
                                                     
@@ -1018,26 +2225,68 @@ val is_fields_contents_within_limit2_lemma : (h_index: hp_addr) ->
                                                                  
                             (ensures (is_fields_contents_within_limit2 h_index wz g == true <==>
                                       is_fields_contents_within_limit2 h_index wz' g' == true))
-                            (decreases (Usize.v wz))
+                            (decreases (Usize.v wz)) =
+ if (Usize.v wz = 0) then ()
+ else
+ (
+   assert (Usize.v wz > 0);
+   let s = Usize.add h_index (Usize.mul wz mword) in
+   let wz1 = Usize.sub wz 1UL in
+   let wz2 = Usize.sub wz' 1UL in
+   wosize_times_mword_multiple_of_mword wz;
+   assert (Usize.v (Usize.mul wz mword) % Usize.v mword == 0);
 
-val check_all_block_fields_within_limit2 :(g:heap{Seq.length (objects2 0UL g) > 0})->
-                                          (f':seq Usize.t {(forall x. Seq.mem x f' ==> Usize.v x >= 0 /\ Usize.v x < heap_size) /\
+   sum_of_multiple_of_mword_is_multiple_of_mword h_index (Usize.mul wz mword);
+   
+   assert (is_hp_addr s);
+   let succ = read_word g s in
+   let succ' = read_word g' s in
+   if (isPointer s g) then
+   (
+     assert (succ == succ');
+     if Usize.v succ >= Usize.v mword && Usize.v succ < heap_size && is_hp_addr succ then
+          is_fields_contents_within_limit2_lemma h_index wz1 wz2 g g'
+     else
+         ()
+   )
+   else
+   (
+      assert (~(isPointer s g));
+      is_fields_contents_within_limit2_lemma h_index wz1 wz2 g g';
+      assert (is_fields_contents_within_limit2 h_index wz1 g == true <==>
+              is_fields_contents_within_limit2 h_index wz2 g' == true);
+      assert (is_fields_contents_within_limit2 h_index wz g == true <==>
+              is_fields_contents_within_limit2 h_index wz' g' == true);
+      ()
+   )
+ )
+
+
+let rec check_all_block_fields_within_limit2 (g:heap{Seq.length (objects2 0UL g) > 0})
+                                             (f':seq Usize.t {(forall x. Seq.mem x f' ==> Usize.v x >= 0 /\ Usize.v x < heap_size) /\
                                                               (forall x. Seq.mem x f' ==> Usize.v x % Usize.v mword == 0) /\
                                                                (forall x. Seq.mem x f' ==> 
                                                                  Seq.mem x (get_allocated_block_addresses g)) /\
-                                                               (forall x. Seq.mem x f' ==> is_fields_within_limit1 x (getWosize (read_word g x)))})->
-                               Tot (b: bool{b == true <==> (forall x. Seq.mem x f' ==> 
+                                                               (forall x. Seq.mem x f' ==> is_fields_within_limit1 x (getWosize (read_word g x)))})
+                               :Tot (b: bool{b == true <==> (forall x. Seq.mem x f' ==> 
                                             is_fields_contents_within_limit2 x (getWosize (read_word g x)) g)})
-                                (decreases length f')
+                                (decreases length f') =
+   match length f' with
+   | 0 -> true
+   | _ -> assert (length f' > 0);
+         let hd = Seq.head f' in
+         let tl = Seq.tail f' in
+         assert (Usize.v hd % Usize.v mword == 0);
+         let wz = getWosize (read_word g hd) in
+         if (is_fields_contents_within_limit2 hd wz g) then
+            (
+               assert (is_fields_contents_within_limit2 hd wz g);
+               check_all_block_fields_within_limit2 g tl
+            )
+            else
+             false
+             
+               
 
 
-
-#restart-solver
-
-#restart-solver
-
-#push-options "--split_queries always"
-
-
-#restart-solver 
 
