Proofs/Spec.GC_part02_01.fsti
@@ -22,20 +22,21 @@ module G = Spec.Graph3
 //DFS module
 module D = DFS2
 
+#reset-options "--z3rlimit 100"
 
-val check_all_block_fields_within_limit2_lemma :(g:heap{Seq.length (objects2 0UL g) > 0})->
-                                                (g':heap{Seq.length (objects2 0UL g') > 0})->
+let rec check_all_block_fields_within_limit2_lemma  (g:heap{Seq.length (objects2 0UL g) > 0})
+                                                (g':heap{Seq.length (objects2 0UL g') > 0})
                                                 (f':seq Usize.t {(forall x. Seq.mem x f' ==> Usize.v x >= 0 /\ Usize.v x < heap_size) /\
                                                                  (forall x. Seq.mem x f' ==> Usize.v x % Usize.v mword == 0) /\
                                                                  (forall x. Seq.mem x f' ==> Seq.mem x (get_allocated_block_addresses g)) /\
 
-                                                                 (forall x. Seq.mem x f' ==> is_fields_within_limit1 x (getWosize (read_word g x)))})->
+                                                                 (forall x. Seq.mem x f' ==> is_fields_within_limit1 x (getWosize (read_word g x)))})
                                                 (f'':seq Usize.t {(forall x. Seq.mem x f'' ==> Usize.v x >= 0 /\ Usize.v x < heap_size) /\
                                                                   (forall x. Seq.mem x f'' ==> Usize.v x % Usize.v mword == 0) /\
                                                                   (forall x. Seq.mem x f'' ==> Seq.mem x (get_allocated_block_addresses g')) /\
 
-                                                                  (forall x. Seq.mem x f'' ==> is_fields_within_limit1 x (getWosize (read_word g x)))})->
-                                  Lemma
+                                                                  (forall x. Seq.mem x f'' ==> is_fields_within_limit1 x (getWosize (read_word g x)))})
+                                : Lemma
 
                                   (requires (f' == f'')  /\
                                             (objects2 0UL g ==
@@ -49,7 +50,49 @@ val check_all_block_fields_within_limit2_lemma :(g:heap{Seq.length (objects2 0UL
                                                              read_word g y == read_word g' y))
                                   (ensures check_all_block_fields_within_limit2 g f' == true <==>
                                            check_all_block_fields_within_limit2 g' f'' == true)
-                                   (decreases length f')
+                                   (decreases length f') =
+ match length f' with
+   | 0 -> ()
+   | _ -> assert (length f' > 0);
+         let hd = Seq.head f' in
+         let hd' = Seq.head f'' in
+
+
+         let tl = Seq.tail f' in
+         let tl' = Seq.tail f'' in
+
+
+
+         let wz = getWosize (read_word g hd) in
+         let wz' = getWosize (read_word g' hd') in
+
+         assert (Usize.v hd % Usize.v mword == 0);
+         assert (Usize.v hd' % Usize.v mword == 0);
+
+         assert (wz == wz');
+
+         assert (forall (i:Usize.t {Usize.v i > 0 /\ Usize.v i <= Usize.v wz}). Usize.v (Usize.add hd (Usize.mul i mword)) < heap_size);
+
+         h_index_field_index_all_mword_multiple_lemma1 g hd;
+         assert (forall (i:Usize.t {Usize.v i > 0 /\ Usize.v i <= Usize.v wz}). Usize.v (Usize.add hd (Usize.mul i mword)) % Usize.v mword == 0);
+         assert (forall (i:Usize.t {Usize.v i > 0 /\ Usize.v i <= Usize.v wz}).
+                                                    (*(is_hp_addr ((Usize.add h_index (Usize.mul i mword)))) /\ (*Mandatory condition, since z3 is not detecting modular
+                                                                                                               arithmetic conditions*)
+                                                    isPointer (Usize.add h_index (Usize.mul i mword)) g ==>*)
+                                                    Usize.v (read_word g (Usize.add hd (Usize.mul i mword))) ==
+                                                    Usize.v (read_word g' (Usize.add hd (Usize.mul i mword))));
+
+         is_fields_contents_within_limit2_lemma hd wz wz' g g';
+
+         if (is_fields_contents_within_limit2 hd wz g) then
+            (
+
+               check_all_block_fields_within_limit2_lemma g g' tl tl';
+               ()
+            )
+         else
+           ()
+
 
 
 #restart-solver
@@ -59,7 +102,7 @@ val check_all_block_fields_within_limit2_lemma :(g:heap{Seq.length (objects2 0UL
 #restart-solver
 
 
-let test21  (h_index: hp_addr)
+(*let test21  (h_index: hp_addr)
             (g:heap)
             (wz: wosize{(is_fields_within_limit1 h_index wz /\
                          is_fields_contents_within_limit2 h_index wz g)})
@@ -82,6 +125,8 @@ let test21  (h_index: hp_addr)
  assert (is_hp_addr f_val);
  let h_index' = hd_address (f_val) in
  admit()
+*)
+
 
 let is_fields_points_to_blocks2_post_condition    (h_index: hp_addr)
                                                   (g:heap{Seq.length (objects2 0UL g) > 0})
@@ -117,34 +162,373 @@ let is_fields_points_to_blocks2_post_condition    (h_index: hp_addr)
  ))
 
 
-val is_fields_points_to_blocks2 :    (h_index: hp_addr) ->
-                                     (g:heap{Seq.length (objects2 0UL g) > 0})->
-                                     (wz: wosize{(is_fields_within_limit1 h_index wz /\
-                                               is_fields_contents_within_limit2 h_index wz g)}) ->
-                                     (f':seq Usize.t { (forall x. Seq.mem x f' ==> is_hp_addr x) /\
-                                                    (forall x. Seq.mem x f' ==>
-                                                     Seq.mem x (get_allocated_block_addresses g))})->
-
-                   Tot (b:bool{b == true <==> is_fields_points_to_blocks2_post_condition h_index g wz f'})
-                   (decreases (Usize.v wz))
 
 #restart-solver
 
-val is_fields_points_to_blocks2_lemma : (h_index: hp_addr) ->
-                                        (g:heap{Seq.length (objects2 0UL g) > 0})->
+#reset-options "--z3rlimit 50 --max_fuel 0 --max_ifuel 0 --using_facts_from '* -FStar.Seq'"
+
+let rec is_fields_points_to_blocks2_test      (h_index: hp_addr)
+                                          (g:heap{Seq.length (objects2 0UL g) > 0})
+                                          (wz: wosize{(is_fields_within_limit1 h_index wz /\
+                                               is_fields_contents_within_limit2 h_index wz g)})
+                                          (f':seq Usize.t { (forall x. Seq.mem x f' ==> is_hp_addr x) /\
+                                                    (forall x. Seq.mem x f' ==>
+                                                     Seq.mem x (get_allocated_block_addresses g))})
+
+                   : Tot (b:bool{b == true <==> is_fields_points_to_blocks2_post_condition h_index g wz f'})
+                    (decreases (Usize.v wz)) =
+ assert (is_hp_addr h_index);
+ if (Usize.v wz = 0) then true
+  else
+  (
+    assert (Usize.v wz > 0);
+    //get the successor_index = h_index + wz * mword
+    let s = Usize.add h_index (Usize.mul wz mword) in
+    // For recursing, find wz' = wz - 1
+    let wz' = Usize.sub wz 1UL in
+    wosize_times_mword_multiple_of_mword wz;
+    assert (Usize.v (Usize.mul wz mword) % Usize.v mword == 0);
+    assert ((Usize.v h_index + (Usize.v wz * Usize.v mword)) % Usize.v mword == 0);
+    assert (Usize.v s % Usize.v mword == 0);
+    assert (Usize.v s < heap_size);
+    assert (is_hp_addr s);
+    if (isPointer s g) then
+    (
+
+      lemma_len_slice g (Usize.v s) ((Usize.v s) + (Usize.v mword));
+      let succ = read_word g s in
+      assert (Usize.v succ >= Usize.v mword);
+      assert (Usize.v succ < heap_size);
+      assert (Usize.v succ % Usize.v mword == 0);
+      assert (is_hp_addr succ);
+    //Get the header of succ. succ_hdr = succ - mword
+      let hdr_succ = hd_address succ in
+      let tg = tag_of_object1 hdr_succ g in
+      if (Usize.v tg <> infix_tag) then
+      (
+        assert (Usize.v tg <> infix_tag);
+        if (Seq.mem hdr_succ (get_allocated_block_addresses g)) then
+        (
+          is_fields_points_to_blocks2_test h_index g wz' f'
+        )
+        else
+        (
+          false
+        )
+      )
+      else
+      (
+        assert (Usize.v tg == infix_tag);
+        let wz_succ = wosize_of_object1 hdr_succ g in
+        let wz_succ_offset = Usize.mul wz_succ mword in
+        if (UInt.fits (Usize.v succ - Usize.v wz_succ_offset) Usize.n) then
+        (
+          let actual_succ = Usize.sub succ wz_succ_offset in
+          if (Usize.v actual_succ >= Usize.v mword && is_hp_addr actual_succ) then
+          (
+            let hdr_actual_succ = hd_address actual_succ in
+            let tg_actual = tag_of_object1 hdr_actual_succ g in
+            if (Usize.v tg_actual = closure_tag && Seq.mem hdr_actual_succ (get_allocated_block_addresses g)) then
+            (
+              is_fields_points_to_blocks2_test h_index g wz' f'
+            )
+            else
+            (
+              false
+            )
+          )
+          else
+          (
+            false
+          )
+        )
+        else
+        (
+          false
+        )
+      )
+
+    )
+    else
+    (
+      assert (~(isPointer s g));
+      let b = is_fields_points_to_blocks2_test h_index g wz' f' in
+      b
+    )
+
+  )
+
+
+let rec is_fields_points_to_blocks2 (h_index: hp_addr) 
+                                    (g:heap{Seq.length (objects2 0UL g) > 0})
+                                    (wz: wosize{(is_fields_within_limit1 h_index wz /\
+                                               is_fields_contents_within_limit2 h_index wz g)}) 
+                                    (f':seq Usize.t { (forall x. Seq.mem x f' ==> is_hp_addr x) /\
+                                                    (forall x. Seq.mem x f' ==>
+                                                     Seq.mem x (get_allocated_block_addresses g))})
+
+                  : Tot (b:bool{b == true <==> is_fields_points_to_blocks2_post_condition h_index g wz f'})
+                   (decreases (Usize.v wz)) =
+assert (is_hp_addr h_index);
+ if (Usize.v wz = 0) then true
+  else
+  (
+    assert (Usize.v wz > 0);
+    //get the successor_index = h_index + wz * mword
+    let s = Usize.add h_index (Usize.mul wz mword) in
+    // For recursing, find wz' = wz - 1
+    let wz' = Usize.sub wz 1UL in
+    wosize_times_mword_multiple_of_mword wz;
+    assert (Usize.v (Usize.mul wz mword) % Usize.v mword == 0);
+    assert ((Usize.v h_index + (Usize.v wz * Usize.v mword)) % Usize.v mword == 0);
+    assert (Usize.v s % Usize.v mword == 0);
+    assert (Usize.v s < heap_size);
+    assert (is_hp_addr s);
+    if (isPointer s g) then
+    (
+
+      lemma_len_slice g (Usize.v s) ((Usize.v s) + (Usize.v mword));
+      let succ = read_word g s in
+      assert (Usize.v succ >= Usize.v mword);
+      assert (Usize.v succ < heap_size);
+      assert (Usize.v succ % Usize.v mword == 0);
+      assert (is_hp_addr succ);
+    //Get the header of succ. succ_hdr = succ - mword
+      let hdr_succ = hd_address succ in
+      let tg = tag_of_object1 hdr_succ g in
+      if (Usize.v tg <> infix_tag) then
+      (
+        assert (Usize.v tg <> infix_tag);
+        if (Seq.mem hdr_succ (get_allocated_block_addresses g)) then
+        (
+          is_fields_points_to_blocks2 h_index g wz' f'
+        )
+        else
+        (
+          false
+        )
+      )
+      else
+      (
+        assert (Usize.v tg == infix_tag);
+        let wz_succ = wosize_of_object1 hdr_succ g in
+        let wz_succ_offset = Usize.mul wz_succ mword in
+        if (UInt.fits (Usize.v succ - Usize.v wz_succ_offset) Usize.n) then
+        (
+          let actual_succ = Usize.sub succ wz_succ_offset in
+          if (Usize.v actual_succ >= Usize.v mword && is_hp_addr actual_succ) then
+          (
+            let hdr_actual_succ = hd_address actual_succ in
+            let tg_actual = tag_of_object1 hdr_actual_succ g in
+            if (Usize.v tg_actual = closure_tag && Seq.mem hdr_actual_succ (get_allocated_block_addresses g)) then
+            (
+              is_fields_points_to_blocks2 h_index g wz' f'
+            )
+            else
+            (
+              false
+            )
+          )
+          else
+          (
+            false
+          )
+        )
+        else
+        (
+          false
+        )
+      )
+
+    )
+    else
+    (
+      assert (~(isPointer s g));
+      let b = is_fields_points_to_blocks2 h_index g wz' f' in
+      b
+    )
+
+  )
+
+
+#restart-solver
+
+#restart-solver
+
+#restart-solver
+
+#reset-options "--z3rlimit 500"
+
+#push-options "--split_queries always"
+
+#restart-solver
+
+let rec is_fields_points_to_blocks2_lemma1  (h_index: hp_addr)
+                                        (g:heap{Seq.length (objects2 0UL g) > 0})
                                         (wz: wosize{(is_fields_within_limit1 h_index wz /\
-                                                     is_fields_contents_within_limit2 h_index wz g)}) ->
+                                                     is_fields_contents_within_limit2 h_index wz g)})
                                         (f':seq Usize.t { (forall x. Seq.mem x f' ==> Usize.v x >= 0 /\ Usize.v x < heap_size) /\
                                                           (forall x. Seq.mem x f' ==> is_hp_addr x) /\
-                                                          (forall x. Seq.mem x f' ==> Seq.mem x (get_allocated_block_addresses g))})->
-                                        (g':heap{Seq.length (objects2 0UL g') > 0})->
-                                        (wz': wosize{(is_fields_within_limit1 h_index wz' /\
-                                                      is_fields_contents_within_limit2 h_index wz' g')}) ->
+                                                          (forall x. Seq.mem x f' ==> Seq.mem x (get_allocated_block_addresses g))})
+                                        (g':heap{Seq.length (objects2 0UL g') > 0})
+                                        (wz1: wosize{(is_fields_within_limit1 h_index wz1 /\
+                                                      is_fields_contents_within_limit2 h_index wz1 g')})
                                         (f'':seq Usize.t { (forall x. Seq.mem x f'' ==> Usize.v x >= 0 /\ Usize.v x < heap_size) /\
                                                            (forall x. Seq.mem x f'' ==> is_hp_addr x) /\
-                                                           (forall x. Seq.mem x f'' ==> Seq.mem x (get_allocated_block_addresses g'))})->
-                                  Lemma
-                                  (requires (wz == wz') /\
+                                                           (forall x. Seq.mem x f'' ==> Seq.mem x (get_allocated_block_addresses g'))})
+                               : Lemma
+                                  (requires (wz == wz1) /\
+                                            (f' == f'')  /\
+                                            (objects2 0UL g == objects2 0UL g') /\
+                                            (get_allocated_block_addresses g == get_allocated_block_addresses g') (*/\
+                                      (forall x. Usize.v x  >= Usize.v h_index + Usize.v mword /\
+                                            Usize.v x <= Usize.v h_index + (Usize.v wz * Usize.v mword) ==>
+                                            (length (slice g' (Usize.v x) ((Usize.v x) + (Usize.v mword))) = 8)) /\
+
+                                      (forall x. Usize.v x  >= Usize.v h_index + Usize.v mword /\
+                                            Usize.v x <= Usize.v h_index + (Usize.v wz * Usize.v mword) ==>
+                                            (length (slice g (Usize.v x) ((Usize.v x) + (Usize.v mword))) = 8))*) /\
+
+                                      (forall (x:Usize.t{Usize.v x < heap_size /\ Usize.v x % 8 == 0}). wosize_of_object1 x g ==
+                                               wosize_of_object1 x g') /\
+                                      (forall (x:Usize.t{Usize.v x < heap_size /\ Usize.v x % 8 == 0}). tag_of_object1 x g ==
+                                               tag_of_object1 x g') /\
+
+                                      (forall x. Usize.v x  >= Usize.v h_index + Usize.v mword /\
+                                            Usize.v x <= Usize.v h_index + (Usize.v wz * Usize.v mword) ==> read_word g x == read_word g' x))
+                                  (ensures is_fields_points_to_blocks2 h_index g wz f' == true <==>
+                                            is_fields_points_to_blocks2 h_index g' wz1 f'' == true)
+                                  (decreases (Usize.v wz)) =
+ if (Usize.v wz = 0) then ()
+  else
+  (
+    assert (Usize.v wz > 0);
+        //get the successor_index = h_index + wz * mword
+    let s = Usize.add h_index (Usize.mul wz mword) in
+
+    // For recursing, find wz' = wz - 1
+    let wz' = Usize.sub wz 1UL in
+    let wz2 = Usize.sub wz1 1UL in
+
+    wosize_times_mword_multiple_of_mword wz;
+    assert (Usize.v (Usize.mul wz mword) % Usize.v mword == 0);
+
+    sum_of_multiple_of_mword_is_multiple_of_mword h_index (Usize.mul wz mword);
+    assert ((Usize.v h_index + (Usize.v wz * Usize.v mword)) % Usize.v mword == 0);
+    assert (Usize.v s % Usize.v mword == 0);
+    assert (Usize.v s < heap_size);
+    assert (is_hp_addr s);
+    if (isPointer s g) then
+    (
+      let succ = read_word g s in
+      let succ' = read_word g' s in
+      assert (succ == succ');
+
+      assert (Usize.v succ >= Usize.v mword);
+      assert (Usize.v succ < heap_size);
+      assert (Usize.v succ % Usize.v mword == 0);
+      assert (is_hp_addr succ);
+
+      let hdr_succ = hd_address succ in
+      let hdr_succ1 = hd_address succ' in
+      assert (hdr_succ = hdr_succ1);
+      let tg = tag_of_object1 hdr_succ g in
+      let tg1 = tag_of_object1 hdr_succ1 g' in
+      assert (forall (x:Usize.t{Usize.v x < heap_size /\ Usize.v x % 8 == 0}). tag_of_object1 x g ==
+                                               tag_of_object1 x g');
+      assert (Usize.v hdr_succ < heap_size /\ Usize.v hdr_succ % 8 == 0);
+      assert (tg == tg1);
+      if (Usize.v tg <> infix_tag) then
+      (
+        assert (Usize.v tg <> infix_tag);
+        assert (get_allocated_block_addresses g == get_allocated_block_addresses g');
+        if (Seq.mem hdr_succ (get_allocated_block_addresses g)) then
+        (
+          is_fields_points_to_blocks2_lemma1 h_index g wz' f' g' wz2 f'';
+          assert (is_fields_points_to_blocks2 h_index g wz' f' == true <==>
+                                            is_fields_points_to_blocks2 h_index g' wz2 f'' == true);
+          ()
+
+        )
+        else
+        (
+          ()
+        )
+      )
+
+      else
+      (
+        assert (Usize.v tg == infix_tag);
+        let wz_succ = wosize_of_object1 hdr_succ g in
+        let wz_succ1 = wosize_of_object1 hdr_succ1 g' in
+        let wz_succ_offset = Usize.mul wz_succ mword in
+        let wz_succ_offset1 = Usize.mul wz_succ1 mword in
+        assert (forall (x:Usize.t{Usize.v x < heap_size /\ Usize.v x % 8 == 0}). wosize_of_object1 x g ==
+                                               wosize_of_object1 x g');
+        assert (wz_succ == wz_succ1);
+        if (UInt.fits (Usize.v succ - Usize.v wz_succ_offset) Usize.n) then
+        (
+          let actual_succ = Usize.sub succ wz_succ_offset in
+          let actual_succ1 = Usize.sub succ' wz_succ_offset1 in
+          if (Usize.v actual_succ >= Usize.v mword && is_hp_addr actual_succ) then
+          (
+             let hdr_actual_succ = hd_address actual_succ in
+             let hdr_actual_succ1 = hd_address actual_succ1 in
+             let tg_actual = tag_of_object1 hdr_actual_succ g in
+             let tg_actual1 = tag_of_object1 hdr_actual_succ1 g' in
+             assert (Usize.v hdr_actual_succ < heap_size /\ Usize.v hdr_actual_succ % 8 == 0);
+             assert (forall (x:Usize.t{Usize.v x < heap_size /\ Usize.v x % 8 == 0}). tag_of_object1 x g ==
+                                               tag_of_object1 x g');
+             assert (tg_actual == tg_actual1);
+            if (Usize.v tg_actual = closure_tag && Seq.mem hdr_actual_succ (get_allocated_block_addresses g)) then
+            (
+               is_fields_points_to_blocks2_lemma1 h_index g wz' f' g' wz2 f'';
+               ()
+            )
+            else
+            (
+              ()
+            )
+          )
+          else
+          (
+            ()
+          )
+        )
+        else
+        (
+          ()
+        )
+      )
+    )
+    else
+    (
+       assert (~(isPointer s g));
+
+       is_fields_points_to_blocks2_lemma1 h_index g wz' f' g' wz2 f'';
+       ()
+    )
+  )
+
+#restart-solver
+
+#restart-solver
+
+let rec is_fields_points_to_blocks2_lemma (h_index: hp_addr) 
+                                          (g:heap{Seq.length (objects2 0UL g) > 0})
+                                          (wz: wosize{(is_fields_within_limit1 h_index wz /\
+                                                     is_fields_contents_within_limit2 h_index wz g)}) 
+                                          (f':seq Usize.t { (forall x. Seq.mem x f' ==> Usize.v x >= 0 /\ Usize.v x < heap_size) /\
+                                                          (forall x. Seq.mem x f' ==> is_hp_addr x) /\
+                                                          (forall x. Seq.mem x f' ==> Seq.mem x (get_allocated_block_addresses g))})
+                                          (g':heap{Seq.length (objects2 0UL g') > 0})
+                                          (wz1: wosize{(is_fields_within_limit1 h_index wz1 /\
+                                                      is_fields_contents_within_limit2 h_index wz1 g')}) 
+                                          (f'':seq Usize.t { (forall x. Seq.mem x f'' ==> Usize.v x >= 0 /\ Usize.v x < heap_size) /\
+                                                           (forall x. Seq.mem x f'' ==> is_hp_addr x) /\
+                                                           (forall x. Seq.mem x f'' ==> Seq.mem x (get_allocated_block_addresses g'))})
+                                  :Lemma
+                                  (requires (wz == wz1) /\
                                             (f' == f'')  /\
                                             (objects2 0UL g == objects2 0UL g') /\
                                             (get_allocated_block_addresses g == get_allocated_block_addresses g') /\
@@ -156,8 +540,119 @@ val is_fields_points_to_blocks2_lemma : (h_index: hp_addr) ->
                                       (forall x. Usize.v x  >= Usize.v h_index + Usize.v mword /\
                                             Usize.v x <= Usize.v h_index + (Usize.v wz * Usize.v mword) ==> read_word g x == read_word g' x))
                                   (ensures is_fields_points_to_blocks2 h_index g wz f' == true <==>
-                                            is_fields_points_to_blocks2 h_index g' wz' f'' == true)
-                                  (decreases (Usize.v wz))
+                                            is_fields_points_to_blocks2 h_index g' wz1 f'' == true)
+                                  (decreases (Usize.v wz)) =
+ if (Usize.v wz = 0) then ()
+  else
+  (
+    assert (Usize.v wz > 0);
+        //get the successor_index = h_index + wz * mword
+    let s = Usize.add h_index (Usize.mul wz mword) in
+
+    // For recursing, find wz' = wz - 1
+    let wz' = Usize.sub wz 1UL in
+    let wz2 = Usize.sub wz1 1UL in
+
+    wosize_times_mword_multiple_of_mword wz;
+    assert (Usize.v (Usize.mul wz mword) % Usize.v mword == 0);
+
+    sum_of_multiple_of_mword_is_multiple_of_mword h_index (Usize.mul wz mword);
+    assert ((Usize.v h_index + (Usize.v wz * Usize.v mword)) % Usize.v mword == 0);
+    assert (Usize.v s % Usize.v mword == 0);
+    assert (Usize.v s < heap_size);
+    assert (is_hp_addr s);
+    if (isPointer s g) then
+    (
+      let succ = read_word g s in
+      let succ' = read_word g' s in
+      assert (succ == succ');
+
+      assert (Usize.v succ >= Usize.v mword);
+      assert (Usize.v succ < heap_size);
+      assert (Usize.v succ % Usize.v mword == 0);
+      assert (is_hp_addr succ);
+
+      let hdr_succ = hd_address succ in
+      let hdr_succ1 = hd_address succ' in
+      assert (hdr_succ = hdr_succ1);
+      let tg = tag_of_object1 hdr_succ g in
+      let tg1 = tag_of_object1 hdr_succ1 g' in
+      assert (forall (x:Usize.t{Usize.v x < heap_size /\ Usize.v x % 8 == 0}). tag_of_object1 x g ==
+                                               tag_of_object1 x g');
+      assert (Usize.v hdr_succ < heap_size /\ Usize.v hdr_succ % 8 == 0);
+      assert (tg == tg1);
+      if (Usize.v tg <> infix_tag) then
+      (
+        assert (Usize.v tg <> infix_tag);
+        assert (get_allocated_block_addresses g == get_allocated_block_addresses g');
+        if (Seq.mem hdr_succ (get_allocated_block_addresses g)) then
+        (
+          is_fields_points_to_blocks2_lemma h_index g wz' f' g' wz2 f'';
+          assert (is_fields_points_to_blocks2 h_index g wz' f' == true <==>
+                                            is_fields_points_to_blocks2 h_index g' wz2 f'' == true);
+          ()
+
+        )
+        else
+        (
+          ()
+        )
+      )
+
+      else
+      (
+        assert (Usize.v tg == infix_tag);
+        let wz_succ = wosize_of_object1 hdr_succ g in
+        let wz_succ1 = wosize_of_object1 hdr_succ1 g' in
+        let wz_succ_offset = Usize.mul wz_succ mword in
+        let wz_succ_offset1 = Usize.mul wz_succ1 mword in
+        assert (forall (x:Usize.t{Usize.v x < heap_size /\ Usize.v x % 8 == 0}). wosize_of_object1 x g ==
+                                               wosize_of_object1 x g');
+        assert (wz_succ == wz_succ1);
+        if (UInt.fits (Usize.v succ - Usize.v wz_succ_offset) Usize.n) then
+        (
+          let actual_succ = Usize.sub succ wz_succ_offset in
+          let actual_succ1 = Usize.sub succ' wz_succ_offset1 in
+          if (Usize.v actual_succ >= Usize.v mword && is_hp_addr actual_succ) then
+          (
+             let hdr_actual_succ = hd_address actual_succ in
+             let hdr_actual_succ1 = hd_address actual_succ1 in
+             let tg_actual = tag_of_object1 hdr_actual_succ g in
+             let tg_actual1 = tag_of_object1 hdr_actual_succ1 g' in
+             assert (Usize.v hdr_actual_succ < heap_size /\ Usize.v hdr_actual_succ % 8 == 0);
+             assert (forall (x:Usize.t{Usize.v x < heap_size /\ Usize.v x % 8 == 0}). tag_of_object1 x g ==
+                                               tag_of_object1 x g');
+             assert (tg_actual == tg_actual1);
+            if (Usize.v tg_actual = closure_tag && Seq.mem hdr_actual_succ (get_allocated_block_addresses g)) then
+            (
+               is_fields_points_to_blocks2_lemma h_index g wz' f' g' wz2 f'';
+               ()
+            )
+            else
+            (
+              ()
+            )
+          )
+          else
+          (
+            ()
+          )
+        )
+        else
+        (
+          ()
+        )
+      )
+    )
+    else
+    (
+       assert (~(isPointer s g));
+
+       is_fields_points_to_blocks2_lemma h_index g wz' f' g' wz2 f'';
+       ()
+    )
+  )
+
 
 let empty_lemma (f:seq Usize.t)
        : Lemma
@@ -185,27 +680,100 @@ let length'_lemma (f:seq Usize.t)
          (ensures length' (Seq.tail f) < length' f) =
  ()
 
+#restart-solver
 
-val check_fields_points_to_blocks2:(g:heap{Seq.length (objects2 0UL g) > 0})->
-                                   (f':seq Usize.t { (forall x. Seq.mem x f' ==> Usize.v x >= 0 /\ Usize.v x < heap_size) /\
+let get_allocated_block_addresses_color_lemma (g:heap {Seq.length (objects2 0UL g) > 0})
+                                              (x:hp_addr{Seq.mem x (objects2 0UL g)})
+                : Lemma
+                  (requires color_of_object1 x g == white)
+                  (ensures (Seq.mem x (get_allocated_block_addresses g))) =
+  assert (forall x. Seq.mem x (objects2 0UL g) /\
+                    ((isWhiteObject1 x g) \/ (isGrayObject1 x g) \/ (isBlackObject1 x g))==>
+                     Seq.mem x (get_allocated_block_addresses g));
+
+  assert (Seq.mem x (get_allocated_block_addresses g));
+  ()
+
+#reset-options "--z3rlimit 500" // --max_fuel 0 --max_ifuel 0 --using_facts_from '* -FStar.Seq'"
+
+#restart-solver
+
+#restart-solver
+
+#restart-solver
+
+let rec check_fields_points_to_blocks2_test (g:heap{Seq.length (objects2 0UL g) > 0})
+                                            (f':seq Usize.t { (forall x. Seq.mem x f' ==> Usize.v x >= 0 /\ Usize.v x < heap_size) /\
                                                      (forall x. Seq.mem x f' ==> is_hp_addr x) /\
                                                      (forall x. Seq.mem x f' ==> Seq.mem x (get_allocated_block_addresses g)) /\
-                                                     check_all_block_fields_within_limit2  g f'}) ->
+                                                     check_all_block_fields_within_limit2  g f'})
 
 
-                               Tot (b:bool{b == true <==> (forall x. Seq.mem x f' ==>
+                               : Tot (b:bool{b == true <==> (forall x. Seq.mem x f' ==>
                                           is_fields_points_to_blocks2 x g (getWosize (read_word g x)) (get_allocated_block_addresses g))})
-                               (decreases length' f')
+                               (decreases length' f')  =
+  match length f' with
+   | 0 -> empty_lemma f';true
+   | _ -> //assert (length f' > 0);
+         non_empty_mem_lemma f';
+         let hd = Seq.head f' in
+         let tl = Seq.tail f' in
+         let wz = getWosize (read_word g hd) in
 
-#restart-solver
+         if Usize.v wz = 0 then
+             check_fields_points_to_blocks2_test g tl
 
-#restart-solver
+         else
+           (
+             assert (Usize.v wz > 0);
+             assert (is_fields_contents_within_limit2 hd (getWosize (read_word g hd)) g);
+             if (is_fields_points_to_blocks2 hd g (getWosize (read_word g hd)) (get_allocated_block_addresses g)) then
+             (
+                 assert (Seq.tail f' == tl);
+                 assert (Seq.length tl < Seq.length f');
+                 length'_lemma f';
+                 check_fields_points_to_blocks2_test g tl
 
-#restart-solver
+             )
+             else
+                  false
 
-#restart-solver
+           )
 
-#restart-solver
+
+let rec check_fields_points_to_blocks2  (g:heap{Seq.length (objects2 0UL g) > 0})
+                                        (f':seq Usize.t { (forall x. Seq.mem x f' ==> Usize.v x >= 0 /\ Usize.v x < heap_size) /\
+                                                     (forall x. Seq.mem x f' ==> is_hp_addr x) /\
+                                                     (forall x. Seq.mem x f' ==> Seq.mem x (get_allocated_block_addresses g)) /\
+                                                     check_all_block_fields_within_limit2  g f'}) 
+
+
+                               :Tot (b:bool{b == true <==> (forall x. Seq.mem x f' ==>
+                                          is_fields_points_to_blocks2 x g (getWosize (read_word g x)) (get_allocated_block_addresses g))})
+                               (decreases length' f') =
+  match length f' with
+   | 0 -> empty_lemma f';true
+   | _ -> assert (length f' > 0);
+         non_empty_mem_lemma f';
+         let hd = Seq.head f' in
+         let tl = Seq.tail f' in
+         let wz = getWosize (read_word g hd) in
+         assert (Usize.v wz > 0);
+
+         assert (is_fields_contents_within_limit2 hd (getWosize (read_word g hd)) g);
+             if (is_fields_points_to_blocks2 hd g (getWosize (read_word g hd)) (get_allocated_block_addresses g)) then
+             (
+                 assert (Seq.tail f' == tl);
+                 assert (Seq.length tl < Seq.length f');
+                 length'_lemma f';
+                 check_fields_points_to_blocks2 g tl
+
+             )
+             else
+                  false
+
+
+
 
 let check_fields_points_to_blocks2_lemma_pre (g:heap{Seq.length (objects2 0UL g) > 0})
                                              (g':heap{Seq.length (objects2 0UL g') > 0})
@@ -222,31 +790,38 @@ let check_fields_points_to_blocks2_lemma_pre (g:heap{Seq.length (objects2 0UL g)
                                                                             Usize.v y <= Usize.v x + (Usize.v (getWosize (read_word g x)) * Usize.v mword) ==>
                                                               read_word g y == read_word g' y)
 
-//#reset-options "--z3rlimit 50 --max_fuel 0 --max_ifuel 0 --using_facts_from '* -FStar.Seq'"
+let seq_length_lemma  (#a:Type)
+                      (f:seq a)
+        : Lemma
+          (requires Seq.length f <> 0)
+          (ensures Seq.length f > 0) =
+()
 
-//#push-options "--split_queries always"
-
+#reset-options "--z3rlimit 500"
 
 #restart-solver
 
-val check_fields_points_to_blocks2_lemma : (g:heap{Seq.length (objects2 0UL g) > 0})->
-                                           (g':heap{Seq.length (objects2 0UL g') > 0}) ->
-                                           (f':seq Usize.t {(forall x. Seq.mem x f' ==> Usize.v x >= 0 /\ Usize.v x < heap_size) /\
+#reset-options "--z3rlimit 50 --max_fuel 0 --max_ifuel 0 --using_facts_from '* -FStar.Seq'"
+
+
+let rec check_fields_points_to_blocks2_lemma   (g:heap{Seq.length (objects2 0UL g) > 0})
+                                               (g':heap{Seq.length (objects2 0UL g') > 0}) 
+                                               (f':seq Usize.t {(forall x. Seq.mem x f' ==> Usize.v x >= 0 /\ Usize.v x < heap_size) /\
                                                            (forall x. Seq.mem x f' ==> is_hp_addr x) /\
                                                            (forall x. Seq.mem x f' ==> Seq.mem x (get_allocated_block_addresses g))  /\
                                                            (forall x. Seq.mem x f' ==>
                                                                    is_fields_contents_within_limit2 x (getWosize (read_word g x)) g)(*/\
-                                                           check_all_block_fields_within_limit2 g f'*)})->
+                                                           check_all_block_fields_within_limit2 g f'*)})
 
 
-                                           (f'':seq Usize.t {(forall x. Seq.mem x f'' ==> Usize.v x >= 0 /\ Usize.v x < heap_size) /\
+                                              (f'':seq Usize.t {(forall x. Seq.mem x f'' ==> Usize.v x >= 0 /\ Usize.v x < heap_size) /\
                                                             (forall x. Seq.mem x f'' ==> is_hp_addr x) /\
                                                             (forall x. Seq.mem x f'' ==> Seq.mem x (get_allocated_block_addresses g'))  /\
                                                            (forall x. Seq.mem x f'' ==>
                                                                    is_fields_contents_within_limit2 x (getWosize (read_word g' x)) g')(*/\
-                                                            check_all_block_fields_within_limit2 g' f''*)})->
+                                                            check_all_block_fields_within_limit2 g' f''*)})
 
-                                          Lemma
+                                         : Lemma
                                            (requires (f' == f'')  /\ (objects2 0UL g == objects2 0UL g') /\
                                                      (get_allocated_block_addresses g == get_allocated_block_addresses g') /\
                                                      (forall (x:Usize.t{Usize.v x < heap_size /\ (Usize.v x % Usize.v mword == 0)}).
@@ -258,7 +833,53 @@ val check_fields_points_to_blocks2_lemma : (g:heap{Seq.length (objects2 0UL g) >
                                                      check_fields_points_to_blocks2_lemma_pre g g' f')
 
                                            (ensures check_fields_points_to_blocks2 g f' == true <==> check_fields_points_to_blocks2 g' f'' == true)
-                                           (decreases length' f')
+                                           (decreases length' f') =
+  match length f' with
+   | 0 -> empty_lemma f';()
+   | _ -> seq_length_lemma f';
+         assert (length f' > 0);
+         non_empty_mem_lemma f';
+         let hd = Seq.head f' in
+         let hd' = Seq.head f'' in
+         let tl = Seq.tail f' in
+         let tl' = Seq.tail f'' in
+         assert (hd == hd');
+         assert (tl == tl');
+         let wz = getWosize (read_word g hd) in
+         let wz1 = getWosize (read_word g' hd) in
+         assert (wz == wz1);
+         assert (Seq.mem hd f');
+
+         assert (Usize.v wz > 0);
+            assert (is_fields_contents_within_limit2 hd (getWosize (read_word g hd)) g);
+            is_fields_points_to_blocks2_lemma hd g wz (get_allocated_block_addresses g) g' wz1 (get_allocated_block_addresses g');
+            assert (is_fields_points_to_blocks2 hd g wz (get_allocated_block_addresses g) == true <==>
+                                            is_fields_points_to_blocks2 hd g' wz1 (get_allocated_block_addresses g') == true);
+            if (is_fields_points_to_blocks2 hd g wz (get_allocated_block_addresses g)) then
+             (
+              assert (is_fields_points_to_blocks2 hd g wz (get_allocated_block_addresses g));
+              assert (is_fields_points_to_blocks2 hd g' wz1 (get_allocated_block_addresses g'));
+              length'_lemma f';
+              let _ = check_fields_points_to_blocks2_lemma g g' tl tl' in
+              assert(check_fields_points_to_blocks2 g tl == true <==> check_fields_points_to_blocks2 g' tl' == true);
+
+              assert (check_fields_points_to_blocks2 g f' == true <==> check_fields_points_to_blocks2 g' f'' == true);
+              ()
+             )
+            else
+             (
+               (*assert (~(is_fields_points_to_blocks2 hd g (getWosize (read_word g hd)) (objects2 0UL g)));
+               assert (check_fields_points_to_blocks2 g f' == true <==> check_fields_points_to_blocks2 g' f'' == true);
+               ()*)
+               ()
+
+             )
+
+
+
+#reset-options "--z3rlimit 500"
+
+#restart-solver
 
 let closure_obj_props1 (g:heap{Seq.length (objects2 0UL g) > 0})
                       (f:seq Usize.t {(forall x. Seq.mem x f ==> Usize.v x >= 0 /\ Usize.v x < heap_size) /\
@@ -273,91 +894,184 @@ Usize.v (wosize_of_object1 x g) >= 2 /\
          Usize.v (extract_start_env_bits (closinfo_val_from_closure_object g (f_address x))) + 1 <= Usize.v (wosize_of_object1 x g) /\
          Usize.v (extract_start_env_bits (closinfo_val_from_closure_object g (f_address x))) >= 1)
 
-val check_well_formed_closure_objs  :(g:heap{Seq.length (objects2 0UL g) > 0})->
+let rec check_well_formed_closure_objs   (g:heap{Seq.length (objects2 0UL g) > 0})
                                      (f:seq Usize.t {(forall x. Seq.mem x f ==> Usize.v x >= 0 /\ Usize.v x < heap_size) /\
                                                               (forall x. Seq.mem x f ==> Usize.v x % Usize.v mword == 0) /\
                                                                (forall x. Seq.mem x f ==>
                                                                  Seq.mem x (get_allocated_block_addresses g)) /\
-                                                               (forall x. Seq.mem x f ==> is_fields_within_limit1 x (getWosize (read_word g x)))})->
-                               Tot (b: bool{b == true <==> closure_obj_props1 g f})
-                                (decreases length f)
+                                                               (forall x. Seq.mem x f ==> is_fields_within_limit1 x (getWosize (read_word g x)))})
+                              : Tot (b: bool{b == true <==> closure_obj_props1 g f})
+                                (decreases length f) =
+ if Seq.length f = 0 then
+    true
+  else
+  (
+    let obj = Seq.head f in
+    let rest_f = Seq.tail f in
+    let tg = tag_of_object1 obj g in
+    let wz = wosize_of_object1 obj g in
+    if (Usize.v tg = closure_tag) then
+    (
+      if (Usize.v wz >= 2) then
+      (
+         let f_addr = f_address obj in
+         assert (Usize.v f_addr >= Usize.v mword /\
+                (Usize.v (tag_of_object1 (hd_address f_addr) g) == closure_tag) /\
+                (Usize.v (wosize_of_object1 (hd_address f_addr) g) >= 2) /\
+                         is_fields_within_limit1 (hd_address f_addr) (wosize_of_object1 (hd_address f_addr) g));
+         let clos_info = closinfo_val_from_closure_object g f_addr in
+         let start_env = extract_start_env_bits clos_info in
+         assert (Usize.v start_env >= Usize.v (extract_start_env_bits (closinfo_val_from_closure_object g f_addr)));
+         if is_hp_addr start_env && Usize.v start_env + 1 <= Usize.v wz && Usize.v start_env >= 1 then
+         (
+           let b = check_well_formed_closure_objs g rest_f in
+           assert (b == true <==> closure_obj_props g rest_f);
+           assert (Usize.v (tag_of_object1 obj g) == closure_tag);
+           assert (Usize.v (wosize_of_object1 obj g) >= 2 /\
+                  is_hp_addr (extract_start_env_bits (closinfo_val_from_closure_object g (f_address obj))) /\
+                  Usize.v (extract_start_env_bits (closinfo_val_from_closure_object g (f_address obj))) <= Usize.v (wosize_of_object1 obj g) /\
+                  Usize.v (extract_start_env_bits (closinfo_val_from_closure_object g (f_address obj))) >= 1);
+           assert (f == Seq.cons obj rest_f);
+           (*assert (forall x. Seq.mem x rest_f ==> Usize.v (tag_of_object1 x g) = closure_tag ==>
+                                       Usize.v (wosize_of_object1 x g) >= 2 /\
+                                       is_hp_addr (extract_start_env_bits (closinfo_val_from_closure_object g (f_address x))) /\
+                                       Usize.v (extract_start_env_bits (closinfo_val_from_closure_object g (f_address x))) + 1 <= Usize.v (wosize_of_object1 x g) /\
+                                       Usize.v (extract_start_env_bits (closinfo_val_from_closure_object g (f_address x))) >= 1);*)
+           assert (b == true <==> closure_obj_props g f);
+           b
+         )
+         else
+         (
+           let b = false in
+           assert (b == true <==> closure_obj_props g f);
+           b
+         )
+      )
+      else
+      (
+        let b = false in
+        assert (b == true <==> closure_obj_props g f);
+        b
+      )
+    )
+    else
+    (
+      let b = check_well_formed_closure_objs g rest_f in
+      assert (b == true <==> closure_obj_props g rest_f);
+      assert (b == true <==> closure_obj_props g f);
+      b
+    )
+  )
 
-val get_succ_address : (g:heap) ->
-                       (h_index: hp_addr)->
+
+let get_succ_address  (g:heap) 
+                       (h_index: hp_addr)
                        (wz: wosize{is_fields_within_limit1 h_index wz /\
-                         is_fields_contents_within_limit2 h_index wz g})->
-             (i:Usize.t {Usize.v i > 0 /\ Usize.v i <= Usize.v wz})->
-         Tot (s:hp_addr{s == Usize.add h_index (Usize.mul i mword) /\
-                          (Usize.v s >= Usize.v mword)})
+                         is_fields_contents_within_limit2 h_index wz g})
+             (i:Usize.t {Usize.v i > 0 /\ Usize.v i <= Usize.v wz})
+         :Tot (s:hp_addr{s == Usize.add h_index (Usize.mul i mword) /\
+                          (Usize.v s >= Usize.v mword)}) =
+ let succ_address = Usize.add h_index (Usize.mul i mword) in
+ assert (is_hp_addr succ_address);
+ assert (Usize.v succ_address >= Usize.v mword);
+ succ_address
 
 #restart-solver
 
-val get_succ_value : (g:heap)->
-                     (h_index: hp_addr)->
+let get_succ_value   (g:heap)
+                     (h_index: hp_addr)
                      (wz: wosize{is_fields_within_limit1 h_index wz /\
-                               is_fields_contents_within_limit2 h_index wz g})->
-                     (i:Usize.t {Usize.v i > 0 /\ Usize.v i <= Usize.v wz})->
-             Tot (s_val:Usize.t{s_val == read_word g (get_succ_address g h_index wz i)})
+                               is_fields_contents_within_limit2 h_index wz g})
+                     (i:Usize.t {Usize.v i > 0 /\ Usize.v i <= Usize.v wz})
+            : Tot (s_val:Usize.t{s_val == read_word g (get_succ_address g h_index wz i)}) =
+let succ_val = read_word g (get_succ_address g h_index wz i) in
+ succ_val
 
 
-val isPointer_succ : (g:heap)->
-                     (h_index: hp_addr)->
+let isPointer_succ   (g:heap)
+                     (h_index: hp_addr)
                      (wz: wosize{is_fields_within_limit1 h_index wz /\
-                               is_fields_contents_within_limit2 h_index wz g})->
-                     (i:Usize.t {Usize.v i > 0 /\ Usize.v i <= Usize.v wz})->
-            Tot (b:bool{b == true <==> isPointer (get_succ_address g h_index wz i) g})
+                               is_fields_contents_within_limit2 h_index wz g})
+                     (i:Usize.t {Usize.v i > 0 /\ Usize.v i <= Usize.v wz})
+            :Tot (b:bool{b == true <==> isPointer (get_succ_address g h_index wz i) g}) =
+  isPointer (get_succ_address g h_index wz i) g
 
 
-val hdr_address_succ_ptr :  (g:heap)->
-                            (h_index: hp_addr)->
+let hdr_address_succ_ptr    (g:heap)
+                            (h_index: hp_addr)
                             (wz: wosize{is_fields_within_limit1 h_index wz /\
-                               is_fields_contents_within_limit2 h_index wz g})->
+                               is_fields_contents_within_limit2 h_index wz g})
                             (i:Usize.t {(Usize.v i > 0 /\ Usize.v i <= Usize.v wz) /\
-                                      isPointer_succ g h_index wz i})->
-              Tot (hdr_addr:hp_addr{hdr_addr == hd_address (get_succ_value g h_index wz i)})
+                                      isPointer_succ g h_index wz i})
+             : Tot (hdr_addr:hp_addr{hdr_addr == hd_address (get_succ_value g h_index wz i)}) =
+  hd_address (get_succ_value g h_index wz i)
 
-val  wosize_succ : (g:heap)->
-                   (h_index: hp_addr)->
+let  wosize_succ  (g:heap)
+                   (h_index: hp_addr)
                    (wz: wosize{is_fields_within_limit1 h_index wz /\
-                               is_fields_contents_within_limit2 h_index wz g})->
+                               is_fields_contents_within_limit2 h_index wz g})
                    (i:Usize.t {(Usize.v i > 0 /\ Usize.v i <= Usize.v wz) /\
-                                      isPointer_succ g h_index wz i})->
-         Tot (wz_succ:wosize{wz_succ == wosize_of_object1 (hdr_address_succ_ptr g h_index wz i) g})
+                                      isPointer_succ g h_index wz i})
+        : Tot (wz_succ:wosize{wz_succ == wosize_of_object1 (hdr_address_succ_ptr g h_index wz i) g}) =
+ wosize_of_object1 (hdr_address_succ_ptr g h_index wz i) g
 
-val tag_succ : (g:heap)->
-               (h_index: hp_addr)->
+
+let tag_succ   (g:heap)
+               (h_index: hp_addr)
                (wz: wosize{is_fields_within_limit1 h_index wz /\
-                               is_fields_contents_within_limit2 h_index wz g})->
+                               is_fields_contents_within_limit2 h_index wz g})
                (i:Usize.t {(Usize.v i > 0 /\ Usize.v i <= Usize.v wz) /\
-                                      isPointer_succ g h_index wz i})->
-         Tot (tg_succ:wosize{tg_succ == tag_of_object1 (hdr_address_succ_ptr g h_index wz i) g})
+                                      isPointer_succ g h_index wz i})
+         :Tot (tg_succ:wosize{tg_succ == tag_of_object1 (hdr_address_succ_ptr g h_index wz i) g}) =
+ tag_of_object1 (hdr_address_succ_ptr g h_index wz i) g
 
-val infix_sub_wosize_fits : (g:heap)->
-                            (h_index: hp_addr)->
+
+let infix_sub_wosize_fits   (g:heap)
+                            (h_index: hp_addr)
                             (wz: wosize{is_fields_within_limit1 h_index wz /\
-                                      is_fields_contents_within_limit2 h_index wz g}) ->
+                                      is_fields_contents_within_limit2 h_index wz g}) 
                             (i:Usize.t {(Usize.v i > 0 /\ Usize.v i <= Usize.v wz) /\
-                                      isPointer_succ g h_index wz i})->
-             Tot (b:bool{b== true <==> UInt.fits (Usize.v (get_succ_value g h_index wz i) - (Usize.v (wosize_succ g h_index wz i) * Usize.v mword)) Usize.n})
+                                      isPointer_succ g h_index wz i})
+             :Tot (b:bool{b== true <==> 
+                            UInt.fits (Usize.v (get_succ_value g h_index wz i) - (Usize.v (wosize_succ g h_index wz i) * Usize.v mword)) Usize.n}) =
+ (*get the wosize of the header of the succ value*)
+ let wz_succ = wosize_succ g h_index wz i in
+ (*read the succ value*)
+ let succ_val = get_succ_value g h_index wz i in
+ (* prdct = wosize stored in the header of the succ * mword*)
+ let prdct = Usize.v wz_succ * Usize.v mword in
+ (*succ - prdct*)
+ let diff = Usize.v succ_val - prdct in
+ UInt.fits diff Usize.n
 
-val infix_parent : (g:heap)->
-                   (h_index: hp_addr)->
+
+(*closure parent of infix object*)
+(*arguments - h_index wz i g ---> Given an h_index infix parent() finds the closure parent by sustracting the succ value stored at the ith succ from the wosize
+ of that succ header multiplied with mword*)
+
+let infix_parent  (g:heap)
+                   (h_index: hp_addr)
                    (wz: wosize{is_fields_within_limit1 h_index wz /\
-                            is_fields_contents_within_limit2 h_index wz g})->
+                            is_fields_contents_within_limit2 h_index wz g})
                    (i:Usize.t {(Usize.v i > 0 /\ Usize.v i <= Usize.v wz) /\
                                       (isPointer_succ g h_index wz i) /\
-                                      (infix_sub_wosize_fits g h_index wz i)})->
-             Tot (pr_succ: hp_addr{pr_succ == Usize.sub (get_succ_value g h_index wz i) (Usize.mul (wosize_succ g h_index wz i) mword)})
+                                      (infix_sub_wosize_fits g h_index wz i)})
+            : Tot (pr_succ: hp_addr{pr_succ == 
+                              Usize.sub (get_succ_value g h_index wz i) (Usize.mul (wosize_succ g h_index wz i) mword)}) =
+Usize.sub (get_succ_value g h_index wz i) (Usize.mul (wosize_succ g h_index wz i) mword)
 
-val hdr_infix_parent : (g:heap)->
-                       (h_index: hp_addr)->
+(*header address of the parent of the infix object*)
+let hdr_infix_parent   (g:heap)
+                       (h_index: hp_addr)
                        (wz: wosize{is_fields_within_limit1 h_index wz /\
-                            is_fields_contents_within_limit2 h_index wz g})->
+                            is_fields_contents_within_limit2 h_index wz g})
                        (i:Usize.t {(Usize.v i > 0 /\ Usize.v i <= Usize.v wz) /\
                                       (isPointer_succ g h_index wz i) /\
                                       (infix_sub_wosize_fits g h_index wz i) /\
-                                      (Usize.v (infix_parent g h_index wz i) >= Usize.v mword)})->
-             Tot (hdr_pr_succ: hp_addr{hdr_pr_succ == hd_address (infix_parent g h_index wz i)})
+                                      (Usize.v (infix_parent g h_index wz i) >= Usize.v mword)})
+            : Tot (hdr_pr_succ: hp_addr{hdr_pr_succ == hd_address (infix_parent g h_index wz i)}) =
+ hd_address (infix_parent g h_index wz i)
+
 
 let diff_of_multiple_of_mword_is_multiple_of_mword (x:Usize.t{Usize.v x % Usize.v mword == 0})
                                                    (y:Usize.t{Usize.v y % Usize.v mword == 0})
@@ -370,34 +1084,47 @@ let diff_of_multiple_of_mword_is_multiple_of_mword (x:Usize.t{Usize.v x % Usize.
 
 #reset-options "--z3rlimit 500"
 
-val closinfo_val_from_closure_object_lemma : (g:heap)->
+let closinfo_val_from_closure_object_lemma   (g:heap)
                                              (f_addr:hp_addr{Usize.v f_addr >= Usize.v mword /\
                                                     (Usize.v (tag_of_object1 (hd_address f_addr) g) == closure_tag) /\
                                                     (Usize.v (wosize_of_object1 (hd_address f_addr) g) >= 2) /\
                                                     is_fields_within_limit1 (hd_address f_addr) (wosize_of_object1 (hd_address f_addr) g) /\
-                                                    is_fields_contents_within_limit2 (hd_address f_addr) (wosize_of_object1 (hd_address f_addr) g) g})->
-                                             (g':heap)->
-                         Lemma
+                                                    is_fields_contents_within_limit2 (hd_address f_addr) (wosize_of_object1 (hd_address f_addr) g) g})
+                                             (g':heap)
+                        : Lemma
                          (requires (Usize.v f_addr >= Usize.v mword /\
                                    (Usize.v (tag_of_object1 (hd_address f_addr) g') == Usize.v (tag_of_object1 (hd_address f_addr) g)) /\
                                    (Usize.v (wosize_of_object1 (hd_address f_addr) g) == Usize.v (wosize_of_object1 (hd_address f_addr) g')) /\
                                    is_fields_within_limit1 (hd_address f_addr) (wosize_of_object1 (hd_address f_addr) g') /\
                                    read_word g (Usize.add f_addr (Usize.mul 1UL mword)) == read_word g' (Usize.add f_addr (Usize.mul 1UL mword))))
-                         (ensures closinfo_val_from_closure_object g f_addr == closinfo_val_from_closure_object g' f_addr)
+                         (ensures closinfo_val_from_closure_object g f_addr == closinfo_val_from_closure_object g' f_addr) =
+let hdr_f_addr = hd_address f_addr in
+ let offst1 = Usize.mul 1UL mword in
+ let wz = wosize_of_object1 hdr_f_addr g in
+ assert (is_fields_within_limit1 hdr_f_addr wz);
+ let s1 = Usize.add f_addr offst1 in
+ assert (Usize.v s1 < heap_size);
+ assert (Usize.v s1 % Usize.v mword == 0);
+ assert (is_hp_addr s1);
+ let clos_info = read_word g s1 in
+ let clos_info1 = read_word g' s1 in
+ assert (clos_info == clos_info1);
+ ()
 
-val check_well_formed_closure_objs_lemma : (g:heap{Seq.length (objects2 0UL g) > 0})->
-                                           (g':heap{Seq.length (objects2 0UL g') > 0})->
+
+let rec check_well_formed_closure_objs_lemma   (g:heap{Seq.length (objects2 0UL g) > 0})
+                                           (g':heap{Seq.length (objects2 0UL g') > 0})
                                            (f:seq Usize.t {(forall x. Seq.mem x f ==> Usize.v x >= 0 /\ Usize.v x < heap_size) /\
                                                               (forall x. Seq.mem x f ==> Usize.v x % Usize.v mword == 0) /\
                                                                (forall x. Seq.mem x f ==>
                                                                  Seq.mem x (get_allocated_block_addresses g)) /\
-                                                               (forall x. Seq.mem x f ==> is_fields_within_limit1 x (getWosize (read_word g x)))})->
+                                                               (forall x. Seq.mem x f ==> is_fields_within_limit1 x (getWosize (read_word g x)))})
                                            (f'':seq Usize.t {(forall x. Seq.mem x f'' ==> Usize.v x >= 0 /\ Usize.v x < heap_size) /\
                                                                   (forall x. Seq.mem x f'' ==> Usize.v x % Usize.v mword == 0) /\
                                                                   (forall x. Seq.mem x f'' ==> Seq.mem x (get_allocated_block_addresses g')) /\
 
-                                                                  (forall x. Seq.mem x f'' ==> is_fields_within_limit1 x (getWosize (read_word g' x)))})->
-                              Lemma
+                                                                  (forall x. Seq.mem x f'' ==> is_fields_within_limit1 x (getWosize (read_word g' x)))})
+                             : Lemma
                               (requires (f == f'')  /\
                                         (objects2 0UL g == objects2 0UL g') /\
                                         (get_allocated_block_addresses g == get_allocated_block_addresses g') /\
@@ -412,15 +1139,120 @@ val check_well_formed_closure_objs_lemma : (g:heap{Seq.length (objects2 0UL g) >
                                                              read_word g y == read_word g' y))
                                   (ensures check_well_formed_closure_objs g f == true <==>
                                            check_well_formed_closure_objs g' f'' == true)
-                              (decreases length f)
+                              (decreases length f) =
+  if Seq.length f = 0 then
+    ()
+  else
+  (
+    let obj = Seq.head f in
+    let rest_f = Seq.tail f in
+
+    let obj1 = Seq.head f'' in
+    let rest_f1 = Seq.tail f'' in
+
+    assert (obj == obj1);
+    assert (rest_f == rest_f1);
+
+    assert (Seq.length rest_f < Seq.length f);
+
+    let tg = tag_of_object1 obj g in
+    let wz = wosize_of_object1 obj g in
+
+    let tg1 = tag_of_object1 obj g' in
+    let wz1 = wosize_of_object1 obj g' in
+
+    assert (wz == wz1);
+    assert (tg == tg1);
+
+    if (Usize.v tg = closure_tag) then
+    (
+      if (Usize.v wz >= 2) then
+      (
+         let f_addr = f_address obj in
+         assert (Usize.v f_addr >= Usize.v mword /\
+                (Usize.v (tag_of_object1 (hd_address f_addr) g) == closure_tag) /\
+                (Usize.v (wosize_of_object1 (hd_address f_addr) g) >= 2) /\
+                         is_fields_within_limit1 (hd_address f_addr) (wosize_of_object1 (hd_address f_addr) g));
+         let clos_info = closinfo_val_from_closure_object g f_addr in
+         let start_env = extract_start_env_bits clos_info in
+
+         let clos_info1 = closinfo_val_from_closure_object g' f_addr in
+         let start_env1 = extract_start_env_bits clos_info1 in
+
+         assert (clos_info ==  clos_info1);
+         assert (start_env ==  start_env1);
+         assert (Usize.v start_env >= Usize.v (extract_start_env_bits (closinfo_val_from_closure_object g f_addr)));
+         if is_hp_addr start_env && Usize.v start_env <= Usize.v wz && Usize.v start_env >= 1 then
+         (
+           let b = check_well_formed_closure_objs g rest_f in
+
+           check_well_formed_closure_objs_lemma g g' rest_f rest_f1;
+           ()
+         )
+         else
+         (
+           let b = false in
+
+           ()
+         )
+      )
+      else
+      (
+        let b = false in
+
+        ()
+      )
+    )
+    else
+    (
+      let b = check_well_formed_closure_objs g rest_f in
+
+      check_well_formed_closure_objs_lemma g g' rest_f rest_f1;
+      ()
+    )
+  )
 
 
-val well_formed_heap2 : (g:heap) ->
-                 Tot (b:bool{b == true <==> Seq.length (objects2 0UL g) > 0  /\
+let check_well_formed_closure_objs_lemma2_prop  (g:heap{Seq.length (objects2 0UL g) > 0})
+                                                 (f:seq Usize.t {(forall x. Seq.mem x f ==> Usize.v x >= 0 /\ Usize.v x < heap_size) /\
+                                                                  (forall x. Seq.mem x f ==> Usize.v x % Usize.v mword == 0) /\
+                                                                  (forall x. Seq.mem x f ==> Seq.mem x (get_allocated_block_addresses g)) /\
+
+                                                                  (forall x. Seq.mem x f ==> is_fields_within_limit1 x (getWosize (read_word g x)))})=
+  forall x. (Seq.mem x f /\ (Usize.v (tag_of_object1 x g) = closure_tag)) ==>
+                      (Usize.v (wosize_of_object1 x g) >= 2 /\
+                      is_hp_addr (extract_start_env_bits (closinfo_val_from_closure_object g (f_address x))) /\
+                      Usize.v (extract_start_env_bits (closinfo_val_from_closure_object g (f_address x))) + 1 <= Usize.v (wosize_of_object1 x g) /\
+                      Usize.v (extract_start_env_bits (closinfo_val_from_closure_object g (f_address x))) >= 1)
+
+
+#restart-solver
+
+#reset-options "--z3rlimit 100"
+
+
+let well_formed_heap2  (g:heap) 
+                : Tot (b:bool{b == true <==> Seq.length (objects2 0UL g) > 0  /\
                                           (check_all_block_fields_within_limit2 g (get_allocated_block_addresses g)) /\
                                           (check_fields_points_to_blocks2 g (get_allocated_block_addresses g)) /\
                                           (check_well_formed_closure_objs g (get_allocated_block_addresses g))
-                                          })
+                                          }) =
+   let f = objects2 0UL g in
+
+  if length f > 0 then
+  (
+     let f' = get_allocated_block_addresses g in
+     if check_all_block_fields_within_limit2 g f' &&
+        check_fields_points_to_blocks2 g f' &&
+         check_well_formed_closure_objs g f' then
+       true
+     else
+      false
+  )
+
+  else
+   false
+
 
 let is_valid_header1  (h:hp_addr)  // index should be passed to check for header validity
                       (g:heap {well_formed_heap2 g})
